src/cltheory.lean
@@ -5,33 +5,33 @@ universes u v
 namespace fopl
 variables {L : language.{u}} (T : theory L) (i : ℕ)
 
-@[simp] def vecterm.equiv (T : theory L) : ∀ n, vecterm L n → vecterm L n → Prop := λ _ v₁ v₂, T ⊢̇ v₁ ≡̇ v₂
+@[simp] def vecterm.equiv (T : theory L) : ∀ n, vecterm L n → vecterm L n → Prop := λ _ v₁ v₂, T ⊢ v₁ ≡̇ v₂
 
 notation v` ≃[`T :80`] `u:60 := vecterm.equiv T _ v u
 
 @[simp] lemma veq_eq (t u : vecterm L 0) : t ≡̇ u = t =̇ u := rfl
 
-@[simp] lemma vecterm.equiv_refl (T : theory L) : ∀ {n} (v : vecterm L n), T ⊢̇ v ≡̇ v
+@[simp] lemma vecterm.equiv_refl (T : theory L) : ∀ {n} (v : vecterm L n), T ⊢ v ≡̇ v
 | 0     _                  := by simp[vecterm.equiv]
 | (n+1) (vecterm.cons t v) := by { simp[vecterm.equiv], exact vecterm.equiv_refl v}
 
 private lemma vecterm.equiv_symm (T : theory L) : ∀ {n} {v₁ v₂ : vecterm L n},
-  T ⊢̇ v₁ ≡̇ v₂ → T ⊢̇ v₂ ≡̇ v₁
+  T ⊢ v₁ ≡̇ v₂ → T ⊢ v₂ ≡̇ v₁
 | 0     _                    _                    := by simp[vecterm.equiv, provable.eq_symm]
 | (n+1) (vecterm.cons t₁ v₁) (vecterm.cons t₂ v₂) :=
     by { simp[vecterm.equiv, provable.eq_symm], refine λ h₁ h₂, ⟨h₁, vecterm.equiv_symm h₂⟩ }
 
 private lemma vecterm.equiv_trans (T : theory L) : ∀ {n} {v₁ v₂ v₃ : vecterm L n},
-  T ⊢̇ v₁ ≡̇ v₂ → T ⊢̇ v₂ ≡̇ v₃ → T ⊢̇ v₁ ≡̇ v₃
+  T ⊢ v₁ ≡̇ v₂ → T ⊢ v₂ ≡̇ v₃ → T ⊢ v₁ ≡̇ v₃
 | 0     _                 _ _ := by simp[vecterm.equiv]; exact provable.eq_trans
 | (n+1) (vecterm.cons t₁ v₁) (vecterm.cons t₂ v₂) (vecterm.cons t₃ v₃) := 
     by {simp[vecterm.equiv], refine λ e₁ h₁ e₂ h₂, ⟨provable.eq_trans e₁ e₂, vecterm.equiv_trans h₁ h₂⟩ }
 
-theorem vecterm_equiv_equivalence (T : theory L) : equivalence (λ t₁ t₂, T ⊢̇ t₁ =̇ t₂) :=
+theorem vecterm_equiv_equivalence (T : theory L) : equivalence (λ t₁ t₂, T ⊢ t₁ =̇ t₂) :=
 ⟨λ _, by simp, λ _ _ , provable.eq_symm.mp, λ _ _ _, provable.eq_trans⟩
 
 @[reducible, simp, instance]
-def herbrand (n : ℕ) : setoid (term L) := ⟨λ t₁ t₂, T^n ⊢̇ t₁ =̇ t₂, vecterm_equiv_equivalence (T^n)⟩
+def herbrand (n : ℕ) : setoid (term L) := ⟨λ t₁ t₂, T^n ⊢ t₁ =̇ t₂, vecterm_equiv_equivalence (T^n)⟩
 
 def Herbrand (n : ℕ) : Type u := quotient (herbrand T n)
 
@@ -54,24 +54,24 @@ quotient.induction_on' d h
 
 @[elab_as_eliminator, reducible]
 protected def lift_on {φ} (d : Herbrand T i) (f : term L → φ)
-  (h : ∀ v u : term L, T^i ⊢̇ v =̇ u → f v = f u) : φ :=
+  (h : ∀ v u : term L, T^i ⊢ v =̇ u → f v = f u) : φ :=
 quotient.lift_on' d f h
 
 @[simp]
 protected lemma lift_on_eq {φ} (t : term L) (f : term L → φ)
-  (h : ∀ v u, T^i ⊢̇ v =̇ u → f v = f u) : fopl.Herbrand.lift_on (⟦t⟧ᴴ : Herbrand T i) f h = f t := rfl
+  (h : ∀ v u, T^i ⊢ v =̇ u → f v = f u) : fopl.Herbrand.lift_on (⟦t⟧ᴴ : Herbrand T i) f h = f t := rfl
 
 @[elab_as_eliminator, reducible, simp]
 protected def lift_on₂ {φ} (d₁ d₂ : Herbrand T i) (f : term L → term L → φ)
-  (h : ∀ t₁ t₂ u₁ u₂, (T^i ⊢̇ t₁ =̇ u₁) → (T^i ⊢̇ t₂ =̇ u₂) → f t₁ t₂ = f u₁ u₂) : φ :=
+  (h : ∀ t₁ t₂ u₁ u₂, (T^i ⊢ t₁ =̇ u₁) → (T^i ⊢ t₂ =̇ u₂) → f t₁ t₂ = f u₁ u₂) : φ :=
 quotient.lift_on₂' d₁ d₂ f h
 
 @[simp]
 protected lemma lift_on₂_eq {φ} (t u : term L) (f : term L → term L → φ)
-  (h : ∀ t₁ t₂ u₁ u₂, (T^i ⊢̇ t₁ =̇ u₁) → (T^i ⊢̇ t₂ =̇ u₂) → f t₁ t₂ = f u₁ u₂) :
+  (h : ∀ t₁ t₂ u₁ u₂, (T^i ⊢ t₁ =̇ u₁) → (T^i ⊢ t₂ =̇ u₂) → f t₁ t₂ = f u₁ u₂) :
   fopl.Herbrand.lift_on₂ ⟦t⟧ᴴ.T ⟦u⟧ᴴ.T f h = f t u := rfl
 
-lemma of_eq_of {t u : term L} : (⟦t⟧ᴴ : Herbrand T i) = ⟦u⟧ᴴ ↔ (T^i ⊢̇ t =̇ u) :=
+lemma of_eq_of {t u : term L} : (⟦t⟧ᴴ : Herbrand T i) = ⟦u⟧ᴴ ↔ (T^i ⊢ t =̇ u) :=
 by simp[vecterm.quo, vecterm.equiv, quotient.eq']
 
 @[elab_as_eliminator, reducible]
@@ -85,7 +85,7 @@ protected lemma lift_on_vec_eq {φ} {n} (u : dvector (term L) n) (f : dvector (t
 fopl.Herbrand.lift_on_vec ᵥ⟦u⟧ f h = f u := quotient.lift_on_vec_eq u f h
 
 @[simp] lemma equivs_equals : ∀ {n} (v₁ v₂ : dvector (term L) (n+1)),
-  (@setoid.vec_r _ (herbrand T i) _) v₁ v₂ ↔ (T^i ⊢̇ v₁.to_vecterm ≡̇ v₂.to_vecterm)
+  (@setoid.vec_r _ (herbrand T i) _) v₁ v₂ ↔ (T^i ⊢ v₁.to_vecterm ≡̇ v₂.to_vecterm)
 | 0 (t₁ :: dvector.nil) (t₂ :: dvector.nil) := by { simp, refl }
 | (n+1) (t₁ :: v₁) (t₂ :: v₂) := by { simp[equivs_equals v₁ v₂], intros, refl }
 
@@ -103,15 +103,15 @@ def function₂ (T : theory L) (i) (f : L.fn 2) (h₁ h₂ : Herbrand T i) : Her
 notation h₁ ` f⟪` s `⟫² ` h₂ :80 := function₂ _ _ s h₁ h₂
 
 def symbol.pr : ∀ {n} (f : L.pr n), dvector (Herbrand T i) n → Prop
-| 0     c _ := T ⊢̇ formula.const c
-| (n+1) p v := fopl.Herbrand.lift_on_vec v (λ u : dvector (term L) (n+1), T^i ⊢̇ formula.app p (u.to_vecterm))
+| 0     c _ := T ⊢ formula.const c
+| (n+1) p v := fopl.Herbrand.lift_on_vec v (λ u : dvector (term L) (n+1), T^i ⊢ formula.app p (u.to_vecterm))
   $ λ v₁ v₂ eqn, by { simp at*, refine ⟨(provable.e5.MP eqn).MP, (provable.e5.MP (vecterm.equiv_symm _ eqn)).MP⟩  }
 
 def model (T : theory L) : model L := ⟨Herbrand T 0, ⟦#0⟧ᴴ, @symbol.fn _ T 0, @symbol.pr _ T 0⟩
 notation `𝔗[`T`]` := model T
 
-protected theorem provable_iff {t₁ t₂} : T^i ⊢̇ t₁ =̇ t₂ ↔ (⟦t₁⟧ᴴ : Herbrand T i) = ⟦t₂⟧ᴴ := by simp[of_eq_of]
-protected theorem provable_iff0 {t₁ t₂} : T ⊢̇ t₁ =̇ t₂ ↔ (⟦t₁⟧ᴴ : Herbrand T 0) = ⟦t₂⟧ᴴ := by simp[of_eq_of]
+protected theorem provable_iff {t₁ t₂} : T^i ⊢ t₁ =̇ t₂ ↔ (⟦t₁⟧ᴴ : Herbrand T i) = ⟦t₂⟧ᴴ := by simp[of_eq_of]
+protected theorem provable_iff0 {t₁ t₂} : T ⊢ t₁ =̇ t₂ ↔ (⟦t₁⟧ᴴ : Herbrand T 0) = ⟦t₂⟧ᴴ := by simp[of_eq_of]
 
 @[simp] theorem const_function₀_eq {c : L.fn 0} : ⟦vecterm.const c⟧ᴴ = function₀ T i c := rfl
 @[simp] theorem vecterm_app_function₁_eq {f : L.fn 1} {t} : ⟦vecterm.app f t⟧ᴴ = function₁ T i f ⟦t⟧ᴴ := rfl 
@@ -132,13 +132,13 @@ namespace proper
   Herbrand T (i+1) → Herbrand T i :=
 λ h, Herbrand.lift_on h (λ u, ⟦u.rew (ₛ[t]^i)⟧ᴴ : term L → Herbrand T i) $
 λ t₁ t₂ hyp, by { simp[Herbrand.of_eq_of, -provable.iff] at*,
-    have : ordered (T ^ i), from @fopl.ordered_theory_sf_itr _ T fopl.ordered_proper i,
-    have lmm : T^i ⊢̇ t₁ =̇ t₂, exactI provable.inclusion hyp (ordered_inclusion _),
+    have : ordered (T^i), from @fopl.ordered_theory_sf_itr _ T fopl.ordered_proper i,
+    have lmm : T^i ⊢ t₁ =̇ t₂, exactI provable.inclusion hyp (ordered_inclusion _),
     refine provable.ppc_prove_rew i lmm ₛ[t] }
 
 variables [proper 0 T]
 
-def subst_sf_H (i) : Herbrand T 0 → Herbrand T (i+1) → Herbrand T i :=
+def subst_sf_H : Herbrand T 0 → Herbrand T (i+1) → Herbrand T i :=
 λ t h, Herbrand.lift_on t (λ t, subst_sf_H_aux t h : term L → Herbrand T i) $
 λ t₁ t₂ hyp, by { induction h using fopl.Herbrand.ind_on,
   simp[Herbrand.of_eq_of, -provable.iff] at*, 
@@ -148,18 +148,18 @@ def subst_sf_H (i) : Herbrand T 0 → Herbrand T (i+1) → Herbrand T i :=
   { simp[C] }, cases C; simp[C],
   have := provable.sf_itr_sf_itr.mpr hyp, simp at this, refine this }
 notation h₁ ` ⊳ᴴ[`:90 n `] `h₂ :90  := subst_sf_H n h₁ h₂
-notation h₁ ` ⊳ᴴ `h₂ :90  := subst_sf_H _ h₁ h₂
+infix ` ⊳ᴴ ` :90  := subst_sf_H
 
 @[simp] lemma subst_sf_H_function₁ {h₁ : Herbrand T 0} {h₂ : Herbrand T (i+1)} {f} :
   h₁ ⊳ᴴ (function₁ _ _ f h₂) = function₁ _ _ f (h₁ ⊳ᴴ h₂) :=
 by { induction h₁ using fopl.Herbrand.ind_on, induction h₂ using fopl.Herbrand.ind_on,
-     show ⟦h₁⟧ᴴ ⊳ᴴ[i] function₁ T (i + 1) f ⟦h₂⟧ᴴ = function₁ T i f (⟦h₁⟧ᴴ ⊳ᴴ ⟦h₂⟧ᴴ),
+     show ⟦h₁⟧ᴴ ⊳ᴴ function₁ T (i + 1) f ⟦h₂⟧ᴴ = function₁ T i f (⟦h₁⟧ᴴ ⊳ᴴ ⟦h₂⟧ᴴ),
      rw ← vecterm_app_function₁_eq,
      simp[-vecterm_app_function₁_eq, subst_sf_H, Herbrand.of_eq_of], refl }
 
 @[simp] lemma subst_sf_H_function₂
   {h₁ : Herbrand T 0} {h₂ h₃ : Herbrand T (i+1)} {f} :
-  h₁ ⊳ᴴ[i] (function₂ _ _ f h₂ h₃) = function₂ _ _ f (h₁ ⊳ᴴ h₂) (h₁ ⊳ᴴ h₃) :=
+  h₁ ⊳ᴴ (function₂ _ _ f h₂ h₃) = function₂ _ _ f (h₁ ⊳ᴴ h₂) (h₁ ⊳ᴴ h₃) :=
 by { induction h₁ using fopl.Herbrand.ind_on,
      induction h₂ using fopl.Herbrand.ind_on,
      induction h₃ using fopl.Herbrand.ind_on,
@@ -207,28 +207,28 @@ quotient.induction_on' d h
 
 @[elab_as_eliminator, reducible]
 protected def lift_on {φ} (d : Lindenbaum T i) (f : formula L → φ)
-  (h : ∀ p q : formula L, T^i ⊢̇ p ↔̇ q → f p = f q) : φ :=
+  (h : ∀ p q : formula L, T^i ⊢ p ↔̇ q → f p = f q) : φ :=
 quotient.lift_on' d f h
 
 @[simp]
 protected lemma lift_on_eq {φ} (p : formula L) (f : formula L → φ)
-  (h : ∀ p q, T^i ⊢̇ p ↔̇ q → f p = f q) : fopl.Lindenbaum.lift_on ⟦p⟧ᴸ f h = f p := rfl
+  (h : ∀ p q, T^i ⊢ p ↔̇ q → f p = f q) : fopl.Lindenbaum.lift_on ⟦p⟧ᴸ f h = f p := rfl
 
 @[elab_as_eliminator, reducible, simp]
 protected def lift_on₂ {φ} (d₁ d₂ : Lindenbaum T i) (f : formula L → formula L → φ)
-  (h : ∀ p₁ p₂ q₁ q₂, T^i ⊢̇ p₁ ↔̇ q₁ → T^i ⊢̇ p₂ ↔̇ q₂ → f p₁ p₂ = f q₁ q₂) : φ :=
+  (h : ∀ p₁ p₂ q₁ q₂, T^i ⊢ p₁ ↔̇ q₁ → T^i ⊢ p₂ ↔̇ q₂ → f p₁ p₂ = f q₁ q₂) : φ :=
 quotient.lift_on₂' d₁ d₂ f h
 
 @[simp]
 protected lemma lift_on₂_eq {φ} (p q : formula L) (f : formula L → formula L → φ)
-  (h : ∀ p₁ p₂ q₁ q₂, T^i ⊢̇ p₁ ↔̇ q₁ → T^i ⊢̇ p₂ ↔̇ q₂ → f p₁ p₂ = f q₁ q₂) :
+  (h : ∀ p₁ p₂ q₁ q₂, T^i ⊢ p₁ ↔̇ q₁ → T^i ⊢ p₂ ↔̇ q₂ → f p₁ p₂ = f q₁ q₂) :
   fopl.Lindenbaum.lift_on₂ ⟦p⟧ᴸ.T ⟦q⟧ᴸ.T f h = f p q := rfl
 
-protected lemma of_eq_of {p q : formula L} : (⟦p⟧ᴸ : Lindenbaum T i) = ⟦q⟧ᴸ ↔ T^i ⊢̇ p ↔̇ q :=
+protected lemma of_eq_of {p q : formula L} : (⟦p⟧ᴸ : Lindenbaum T i) = ⟦q⟧ᴸ ↔ T^i ⊢ p ↔̇ q :=
 by simp[formula.quo, formula.equiv, quotient.eq']
 
 instance : has_le (Lindenbaum T i) :=
-⟨λ p₁ p₂, Lindenbaum.lift_on₂ p₁ p₂ (λ p₁ p₂, T^i ⊢̇ p₁ →̇ p₂) $
+⟨λ p₁ p₂, Lindenbaum.lift_on₂ p₁ p₂ (λ p₁ p₂, T^i ⊢ p₁ →̇ p₂) $
  λ p₁ p₂ q₁ q₂ hp hq, by { simp at*,
    exact ⟨λ h, (hp.2.imp_trans h).imp_trans hq.1, λ h, (hp.1.imp_trans h).imp_trans hq.2⟩ }⟩
 
@@ -238,26 +238,26 @@ def imply : Lindenbaum T i → Lindenbaum T i → Lindenbaum T i :=
 λ p₁ p₂, Lindenbaum.lift_on₂ p₁ p₂ (λ p₁ p₂, (⟦p₁ →̇ p₂⟧ᴸ : Lindenbaum T i)) $
  λ p₁ p₂ q₁ q₂ hp hq, by { simp[Lindenbaum.of_eq_of] at*, split,
    { refine provable.deduction.mp (provable.deduction.mp _),
-     have : T+{p₁ →̇ p₂}+{q₁} ⊢̇ p₁, from (show _ ⊢̇ q₁ →̇ p₁, by simp[hp]).MP (by simp),
-     have : T+{p₁ →̇ p₂}+{q₁} ⊢̇ p₂, from (show _ ⊢̇ p₁ →̇ p₂, by simp).MP this,
-     exact (show T+{p₁ →̇ p₂}+{q₁} ⊢̇ p₂ →̇ q₂, by simp[hq]).MP this },
+     have : (T^i)+{p₁ →̇ p₂}+{q₁} ⊢ p₁, from (show _ ⊢ q₁ →̇ p₁, by simp[hp]).MP (by simp),
+     have : (T^i)+{p₁ →̇ p₂}+{q₁} ⊢ p₂, from (show _ ⊢ p₁ →̇ p₂, by simp).MP this,
+     exact (show (T^i)+{p₁ →̇ p₂}+{q₁} ⊢ p₂ →̇ q₂, by simp[hq]).MP this },
    { refine provable.deduction.mp (provable.deduction.mp _),
-     have : T+{q₁ →̇ q₂}+{p₁} ⊢̇ q₁, from (show _ ⊢̇ p₁ →̇ q₁, by simp[hp]).MP (by simp),
-     have : T+{q₁ →̇ q₂}+{p₁} ⊢̇ q₂, from (show _ ⊢̇ q₁ →̇ q₂, by simp).MP this,
-     exact (show _ ⊢̇ q₂ →̇ p₂, by simp[hq]).MP this  } }
+     have : (T^i)+{q₁ →̇ q₂}+{p₁} ⊢ q₁, from (show _ ⊢ p₁ →̇ q₁, by simp[hp]).MP (by simp),
+     have : (T^i)+{q₁ →̇ q₂}+{p₁} ⊢ q₂, from (show _ ⊢ q₁ →̇ q₂, by simp).MP this,
+     exact (show _ ⊢ q₂ →̇ p₂, by simp[hq]).MP this } }
 infixr ` ⊑ `:60 := imply
 
 instance : has_inf (Lindenbaum T i) :=
 ⟨λ p₁ p₂, Lindenbaum.lift_on₂ p₁ p₂ (λ p₁ p₂, ⟦p₁ ⩑ p₂⟧ᴸ) $
  λ p₁ p₂ q₁ q₂ hp hq, by { simp[Lindenbaum.of_eq_of] at*, split,
    { apply provable.deduction.mp,
-     have : T+{p₁ ⩑ p₂} ⊢̇ p₁ ⩑ p₂, from provable.add _ _, simp at *,
-     refine ⟨(show T+{p₁ ⩑ p₂} ⊢̇ p₁ →̇ q₁, by simp[hp]).MP this.1,
-       (show T+{p₁ ⩑ p₂} ⊢̇ p₂ →̇ q₂, by simp[hq]).MP this.2⟩ },
+     have : (T^i)+{p₁ ⩑ p₂} ⊢ p₁ ⩑ p₂, from provable.add _ _, simp at *,
+     refine ⟨(show (T^i)+{p₁ ⩑ p₂} ⊢ p₁ →̇ q₁, by simp[hp]).MP this.1,
+       (show (T^i)+{p₁ ⩑ p₂} ⊢ p₂ →̇ q₂, by simp[hq]).MP this.2⟩ },
    { apply provable.deduction.mp,
-     have : T+{q₁ ⩑ q₂} ⊢̇ q₁ ⩑ q₂, from provable.add _ _, simp at *,
-     refine ⟨(show T+{q₁ ⩑ q₂} ⊢̇ q₁ →̇ p₁, by simp[hp]).MP this.1,
-       (show T+{q₁ ⩑ q₂} ⊢̇ q₂ →̇ p₂, by simp[hq]).MP this.2⟩ } }⟩
+     have : (T^i)+{q₁ ⩑ q₂} ⊢ q₁ ⩑ q₂, from provable.add _ _, simp at *,
+     refine ⟨(show (T^i)+{q₁ ⩑ q₂} ⊢ q₁ →̇ p₁, by simp[hp]).MP this.1,
+       (show (T^i)+{q₁ ⩑ q₂} ⊢ q₂ →̇ p₂, by simp[hq]).MP this.2⟩ } }⟩
 
 instance : has_sup (Lindenbaum T i) :=
 ⟨λ p₁ p₂, Lindenbaum.lift_on₂ p₁ p₂ (λ p₁ p₂, ⟦p₁ ⩒ p₂⟧ᴸ) $
@@ -287,23 +287,21 @@ predicate f (h :: dvector.nil)
 def predicate₂ (T : theory L) (i) (f : L.pr 2) (h₁ h₂ : Herbrand T i) : Lindenbaum T i :=
 predicate f (h₁ :: h₂ :: dvector.nil)
 
---notation h₁ ` p⟪` f `⟫² ` h₂ := predicate₂ _ f h₁ h₂
-
 def equal : Herbrand T i → Herbrand T i → Lindenbaum T i :=
 λ h₁ h₂, fopl.Herbrand.lift_on₂ h₁ h₂ (λ t₁ t₂, (⟦t₁ =̇ t₂⟧ᴸ : Lindenbaum T i)) $
 λ t₁ t₂ u₁ u₂ eqn₁ eqn₂, by {
   simp[Lindenbaum.of_eq_of], refine ⟨provable.deduction.mp _, provable.deduction.mp  _⟩,
-  have lmm₁ : (T^i)+{t₁ =̇ t₂} ⊢̇ u₁ =̇ t₁, simp [provable.e2.MP eqn₁],
-  have lmm₂ : (T^i)+{t₁ =̇ t₂} ⊢̇ t₁ =̇ t₂, simp,
-  have lmm₃ : (T^i)+{t₁ =̇ t₂} ⊢̇ t₂ =̇ u₂, simp [eqn₂],
+  have lmm₁ : (T^i)+{t₁ =̇ t₂} ⊢ u₁ =̇ t₁, simp [provable.e2.MP eqn₁],
+  have lmm₂ : (T^i)+{t₁ =̇ t₂} ⊢ t₁ =̇ t₂, simp,
+  have lmm₃ : (T^i)+{t₁ =̇ t₂} ⊢ t₂ =̇ u₂, simp [eqn₂],
   refine (lmm₁.eq_trans lmm₂).eq_trans lmm₃,
-  have lmm₁ : (T^i)+{u₁ =̇ u₂} ⊢̇ t₁ =̇ u₁, simp [eqn₁],
-  have lmm₂ : (T^i)+{u₁ =̇ u₂} ⊢̇ u₁ =̇ u₂, simp,
-  have lmm₃ : (T^i)+{u₁ =̇ u₂} ⊢̇ u₂ =̇ t₂, simp [provable.e2.MP eqn₂],
+  have lmm₁ : (T^i)+{u₁ =̇ u₂} ⊢ t₁ =̇ u₁, simp [eqn₁],
+  have lmm₂ : (T^i)+{u₁ =̇ u₂} ⊢ u₁ =̇ u₂, simp,
+  have lmm₃ : (T^i)+{u₁ =̇ u₂} ⊢ u₂ =̇ t₂, simp [provable.e2.MP eqn₂],
   refine (lmm₁.eq_trans lmm₂).eq_trans lmm₃ }
-infix ` ∥ `:50 := equal
+infix ` ∥ `:60 := equal
 
-def Box : Lindenbaum T i → Prop := λ p, Lindenbaum.lift_on p (λ p, T^i ⊢̇ p) $
+def Box : Lindenbaum T i → Prop := λ p, Lindenbaum.lift_on p (λ p, T^i ⊢ p) $
 λ p₁ p₂ hyp, by { simp at*, refine ⟨λ h, hyp.1.MP h, λ h, hyp.2.MP h⟩ }
 prefix `□`:80 := Box
 
@@ -373,11 +371,11 @@ by induction l using fopl.Lindenbaum.ind_on; simp[has_bot.bot, has_le.le]
 
 lemma mul_le_l (l k : Lindenbaum T i) : l ⊓ k ≤ l :=
 by { induction l using fopl.Lindenbaum.ind_on, induction k using fopl.Lindenbaum.ind_on,
-     simp[has_inf.inf, has_le.le], refine provable.deduction.mp _, have := provable.add T (l ⩑ k), simp* at * }
+     simp[has_inf.inf, has_le.le], refine provable.deduction.mp _, have := provable.add (T^i) (l ⩑ k), simp* at* }
 
 lemma mul_le_r (l k : Lindenbaum T i) : l ⊓ k ≤ k :=
 by { induction l using fopl.Lindenbaum.ind_on, induction k using fopl.Lindenbaum.ind_on,
-     simp[has_inf.inf, has_le.le], refine provable.deduction.mp _, have := provable.add T (l ⩑ k), simp* at * }
+     simp[has_inf.inf, has_le.le], refine provable.deduction.mp _, have := provable.add (T^i) (l ⩑ k), simp* at* }
 
 lemma add_le_l (l k : Lindenbaum T i) : l ≤ l ⊔ k :=
 by { induction l using fopl.Lindenbaum.ind_on, induction k using fopl.Lindenbaum.ind_on,
@@ -412,29 +410,29 @@ by { induction l using fopl.Lindenbaum.ind_on,
      induction n using fopl.Lindenbaum.ind_on,
      simp[has_sup.sup, has_inf.inf, has_le.le, provable.or_r, formula.or],
      refine provable.deduction.mp (provable.deduction.mp _),
-     have lmm₁ : (T^i)+{(¬̇l →̇ m) ⩑ (¬̇l →̇ n)}+{¬̇l} ⊢̇ (¬̇l →̇ m) ⩑ (¬̇l →̇ n), simp[-provable.and],
-     have lmm₂ : (T^i)+{(¬̇l →̇ m) ⩑ (¬̇l →̇ n)}+{¬̇l} ⊢̇ ¬̇l, simp,
+     have lmm₁ : (T^i)+{(¬̇l →̇ m) ⩑ (¬̇l →̇ n)}+{¬̇l} ⊢ (¬̇l →̇ m) ⩑ (¬̇l →̇ n), simp[-provable.and],
+     have lmm₂ : (T^i)+{(¬̇l →̇ m) ⩑ (¬̇l →̇ n)}+{¬̇l} ⊢ ¬̇l, simp,
      simp at lmm₁ ⊢, refine ⟨lmm₁.1.MP lmm₂, lmm₁.2.MP lmm₂⟩ }
 
 private lemma sup_inf_sdiff (l m : Lindenbaum T i) : l ⊓ m ⊔ l ⊓ mᶜ = l :=
 by { induction l using fopl.Lindenbaum.ind_on, induction m using fopl.Lindenbaum.ind_on,
       simp[Lindenbaum.of_eq_of, has_le.le, has_sup.sup, has_inf.inf, has_compl.compl, has_top.top, formula.or],
       refine ⟨contrapose.mp (deduction.mp _), _⟩, simp,
-      have : ∀ n, (T^i)+{¬̇l} ⊢̇ ¬̇(l ⩑ n),
+      have : ∀ n, (T^i)+{¬̇l} ⊢ ¬̇(l ⩑ n),
       { refine λ n, deduction.mpr (contrapose.mpr (deduction.mp _)),
-        have : (T^i)+{l ⩑ n} ⊢̇ l ⩑ n, simp[-provable.and], simp* at* },
+        have : (T^i)+{l ⩑ n} ⊢ l ⩑ n, simp[-provable.and], simp* at* },
       refine ⟨this _, this _⟩,
       refine deduction.mp (deduction.mp _), simp, refine neg_hyp (deduction.mp _),
-      refine explosion (show (T^i)+{l}+{¬̇(l ⩑ m)}+{m} ⊢̇ l ⩑ m, by simp) (by simp) }
+      refine explosion (show (T^i)+{l}+{¬̇(l ⩑ m)}+{m} ⊢ l ⩑ m, by simp) (by simp) }
 
 private lemma inf_inf_sdiff (l m : Lindenbaum T i) : l ⊓ m ⊓ (l ⊓ mᶜ) = ⊥ :=
 by { induction l using fopl.Lindenbaum.ind_on, induction m using fopl.Lindenbaum.ind_on,
      simp[Lindenbaum.of_eq_of, has_le.le, has_sup.sup, has_inf.inf, has_compl.compl, has_bot.bot, formula.or],
-     refine deduction.mp (explosion (show (T^i)+{l ⩑ m ⩑ (l ⩑ ¬̇m)} ⊢̇ m, by simp[axiom_and]) (by simp[axiom_and])) }
+     refine deduction.mp (explosion (show (T^i)+{l ⩑ m ⩑ (l ⩑ ¬̇m)} ⊢ m, by simp[axiom_and]) (by simp[axiom_and])) }
 
 private lemma inf_compl_le_bot (l : Lindenbaum T i) : l ⊓ lᶜ ≤ ⊥ :=
 by { induction l using fopl.Lindenbaum.ind_on, simp[has_le.le, has_inf.inf, has_compl.compl, has_bot.bot],
-     have : (T^i)+{l ⩑ ¬̇l} ⊢̇ l ⩑ ¬̇l, simp[-provable.and], simp at this,
+     have : (T^i)+{l ⩑ ¬̇l} ⊢ l ⩑ ¬̇l, simp[-provable.and], simp at this,
      refine provable.deduction.mp (provable.explosion this.1 this.2) }
 
 private lemma top_le_sup_compl (l : Lindenbaum T i) : ⊤ ≤ l ⊔ lᶜ :=
@@ -469,16 +467,16 @@ instance : boolean_algebra (Lindenbaum T i) :=
   sdiff_eq := λ _ _, rfl }
 
 def fal : Lindenbaum T (i+1) → Lindenbaum T i :=
-λ p, Lindenbaum.lift_on p (λ p, ⟦∀̇p⟧ᴸ) $
+λ p, Lindenbaum.lift_on p (λ p, ⟦∀̇ p⟧ᴸ) $
 λ p₁ p₂ hyp, by { simp[Lindenbaum.of_eq_of] at*, 
   refine ⟨provable.q2.MP (GE hyp.1), provable.q2.MP (GE hyp.2)⟩ }
-prefix `∏`:90 := fal
+prefix `∏ `:90 := fal
 
 def ex : Lindenbaum T (i+1) → Lindenbaum T i :=
-λ p, Lindenbaum.lift_on p (λ p, ⟦∃̇p⟧ᴸ) $
+λ p, Lindenbaum.lift_on p (λ p, ⟦∃̇ p⟧ᴸ) $
 λ p₁ p₂ hyp, by { simp[formula.ex, provable.contrapose, Lindenbaum.of_eq_of] at*, 
   refine ⟨provable.q2.MP $ GE $ contrapose.mpr hyp.1, provable.q2.MP $ GE $ contrapose.mpr hyp.2⟩, }
-prefix `∐`:90 := ex
+prefix `∐ `:90 := ex
 
 def sf : Lindenbaum T i → Lindenbaum T (i+1) :=
 λ p, Lindenbaum.lift_on p (λ p, (⟦p.sf⟧ᴸ : Lindenbaum T (i+1))) $
@@ -489,34 +487,33 @@ namespace proper
 
 variables [proper 0 T]
 
-@[simp] def subst_sf_L_aux (t : term L) (j) :
-  Lindenbaum T (j+i+1) → Lindenbaum T (j+i) :=
-λ p, Lindenbaum.lift_on p (λ p, (⟦p.rew (ₛ[t]^i)⟧ᴸ : Lindenbaum T (j+i))) $
+@[simp] def subst_sf_L_aux (t : term L) :
+  Lindenbaum T (i+1) → Lindenbaum T i :=
+λ p, Lindenbaum.lift_on p (λ p, (⟦p.rew (ₛ[t]^i)⟧ᴸ : Lindenbaum T i)) $
 λ p₁ p₂ hyp, by { simp[Lindenbaum.of_eq_of, -provable.iff] at*,
-    have lmm : T^(j+i) ⊢̇ p₁ ↔̇ p₂, from provable.inclusion hyp (proper_sf_inclusion T (show j+i ≤ j + i + 1, by omega)),
-    have := provable.ppc_prove_rew (j+i) lmm ₛ[t], }
+    have lmm : T^i ⊢ p₁ ↔̇ p₂,
+    { from provable.inclusion hyp (proper_sf_inclusion T (i.le_succ)) },
+    refine provable.ppc_prove_rew i lmm ₛ[t] }
 
-#check @provable.ppc_prove_rew
-
-def subst_sf_L {j} : Herbrand T j → Lindenbaum T (j+i+1) → Lindenbaum T i :=
-λ t l, Herbrand.lift_on t (λ t, subst_sf_L_aux t j l) $
+def subst_sf_L : Herbrand T 0 → Lindenbaum T (i+1) → Lindenbaum T i :=
+λ t l, Herbrand.lift_on t (λ t, subst_sf_L_aux t l) $
 λ t₁ t₂ hyp, by { induction l using fopl.Lindenbaum.ind_on,
   simp[Lindenbaum.of_eq_of, -provable.iff] at*,
   refine equal_rew_iff _ (λ m, _),
-  have C : m < i ∨ m = i ∨ i < m, from trichotomous m i,
+  have C : m < i ∨ m = i ∨ i < m, from trichotomous _ _,
   cases C,
   { simp[C] }, cases C; simp[C],
-  { have := provable.sf_itr_sf_itr.mpr hyp, simp at this, refine this } }
+  { refine provable.sf_itr_sf_itr.mpr hyp } }
 infix ` ⊳ `:90  := subst_sf_L
 
-lemma fal_le_subst_sf_L (l : Lindenbaum T (i+1)) (h) : ∏l ≤ (h ⊳ l) :=
+lemma fal_le_subst_sf_L (l : Lindenbaum T 1) (h) : ∏  l ≤ (h ⊳ l) :=
 begin
   induction l using fopl.Lindenbaum.ind_on with p, 
   induction h using fopl.Herbrand.ind_on with t, 
-  simp[fal, has_le.le, subst_sf_L],
+  simp[fal, has_le.le, subst_sf_L]
 end
 
-lemma subst_sf_L_le_ex (l : Lindenbaum (T^1)) (h) : h ⊳[0] l ≤ ∐l :=
+lemma subst_sf_L_le_ex (l : Lindenbaum T 1) (h) : h ⊳ l ≤ ∐  l :=
 begin
   induction l using fopl.Lindenbaum.ind_on, 
   induction h using fopl.Herbrand.ind_on, 
@@ -526,109 +523,109 @@ begin
   exact provable.q1
 end
 
-@[simp] lemma subst_sf_L_and (h : Herbrand T 0) (n) (l m : Lindenbaum T (i+1)) :
-  h ⊳[n] (l ⊓ m) = h ⊳[n] l ⊓ h ⊳[n] m :=
+@[simp] lemma subst_sf_L_and (h : Herbrand T 0) (l m : Lindenbaum T (i+1)) :
+  h ⊳ (l ⊓ m) = h ⊳ l ⊓ h ⊳ m :=
 by { induction l using fopl.Lindenbaum.ind_on, induction m using fopl.Lindenbaum.ind_on, 
      induction h using fopl.Herbrand.ind_on,
      simp[has_inf.inf, has_le.le, subst_sf_L, Lindenbaum.of_eq_of] }
 
-@[simp] lemma subst_sf_L_or (h : Herbrand T 0) (n) (l m : Lindenbaum T (i+1)) :
-  h ⊳[n] (l ⊔ m) = h ⊳[n] l ⊔ h ⊳[n] m :=
+@[simp] lemma subst_sf_L_or (h : Herbrand T 0) (l m : Lindenbaum T (i+1)) :
+  h ⊳ (l ⊔ m) = h ⊳ l ⊔ h ⊳ m :=
 by { induction l using fopl.Lindenbaum.ind_on, induction m using fopl.Lindenbaum.ind_on, 
      induction h using fopl.Herbrand.ind_on,
      simp[has_sup.sup, has_le.le, subst_sf_L, Lindenbaum.of_eq_of] }
 
-@[simp] lemma subst_sf_L_neg (h : Herbrand T 0) (n) (l : Lindenbaum T (i+1)) :
-  h ⊳[n] lᶜ = (h ⊳[n] l)ᶜ :=
+@[simp] lemma subst_sf_L_neg (h : Herbrand T 0) (l : Lindenbaum T (i+1)) :
+  h ⊳ lᶜ = (h ⊳ l)ᶜ :=
 by { induction l using fopl.Lindenbaum.ind_on,
      induction h using fopl.Herbrand.ind_on,
      simp[has_compl.compl, has_le.le, subst_sf_L, Lindenbaum.of_eq_of] }
 
-@[simp] lemma subst_sf_L_equal (h₁ : Herbrand T) (n) (h₂ h₃ : Herbrand (T^(n+1))) :
-  h₁ ⊳[n] (h₂ ∥ h₃) = (h₁ ⊳ᴴ[n] h₂) ∥ (h₁ ⊳ᴴ[n] h₃) :=
+@[simp] lemma subst_sf_L_equal (h₁ : Herbrand T 0) (h₂ h₃ : Herbrand T (i+1)) :
+  h₁ ⊳ (h₂ ∥ h₃) = (h₁ ⊳ᴴ h₂) ∥ (h₁ ⊳ᴴ h₃) :=
 by { induction h₁ using fopl.Herbrand.ind_on, induction h₂ using fopl.Herbrand.ind_on,
      induction h₃ using fopl.Herbrand.ind_on,
      simp[equal, subst_sf_L, Herbrand.proper.subst_sf_H, Herbrand.proper.subst_sf_H_aux,
        Lindenbaum.of_eq_of] }
 
-@[simp] lemma subst_sf_L_fal (h : Herbrand T 0) (n) (l : Lindenbaum (T^(n+2))) :
-  h ⊳[n] ∏l = ∏(h ⊳[n+1] l) :=
+@[simp] lemma subst_sf_L_fal (h : Herbrand T 0) (l : Lindenbaum T (i+2)) :
+  h ⊳ ∏ l = ∏ (h ⊳ l) :=
 by { induction l using fopl.Lindenbaum.ind_on,
      induction h using fopl.Herbrand.ind_on,
      simp[fal, has_le.le, subst_sf_L, Lindenbaum.of_eq_of, has_pow.pow, rewriting_sf_itr] }
 
-@[simp] lemma subst_sf_L_ex (h : Herbrand T 0) (n) (l : Lindenbaum (T^(n+2))) :
-  h ⊳[n] ∐l = ∐(h ⊳[n+1] l) :=
+@[simp] lemma subst_sf_L_ex (h : Herbrand T 0) (l : Lindenbaum T (i+2)) :
+  h ⊳ ∐ l = ∐ (h ⊳ l) :=
 by { induction l using fopl.Lindenbaum.ind_on,
      induction h using fopl.Herbrand.ind_on,
      simp[ex, has_le.le, subst_sf_L, Lindenbaum.of_eq_of, has_pow.pow, rewriting_sf_itr] }
 
-lemma subst_sf_L_sentence (h : Herbrand T 0) {n} {p : formula L} (a : sentence p) :
-  h ⊳[n] (⟦p⟧ᴸ : Lindenbaum T (i+1)) = ⟦p⟧ᴸ :=
+lemma subst_sf_L_sentence (h : Herbrand T 0) {p : formula L} (a : sentence p) :
+  h ⊳ (⟦p⟧ᴸ : Lindenbaum T (i+1)) = ⟦p⟧ᴸ :=
 by { induction h using fopl.Herbrand.ind_on, simp[subst_sf_L, Lindenbaum.of_eq_of, a] }
 
 end proper
 
-@[simp] lemma prod_top : ∏(⊤ : Lindenbaum T (i+1)) = ⊤ :=
+@[simp] lemma prod_top : ∏ (⊤ : Lindenbaum T (i+1)) = ⊤ :=
 by { simp[fal, has_top.top, Lindenbaum.of_eq_of], apply provable.GE, simp }
 
-lemma provable_GE {l : Lindenbaum T (i+1)} : l = ⊤ → ∏l = ⊤ :=
+lemma provable_GE {l : Lindenbaum T (i+1)} : l = ⊤ → ∏ l = ⊤ :=
 by { induction l using fopl.Lindenbaum.ind_on, simp[fal, has_top.top, Lindenbaum.of_eq_of],
      exact provable.GE }
 
-lemma prenex_ex_neg (l : Lindenbaum T (i+1)) : (∐l)ᶜ = ∏lᶜ :=
+lemma prenex_ex_neg (l : Lindenbaum T (i+1)) : (∐ l)ᶜ = ∏ lᶜ :=
 by induction l using fopl.Lindenbaum.ind_on;
    simp[has_compl.compl, ex, fal, Lindenbaum.of_eq_of, formula.ex]
 
-lemma prenex_fal_neg {l : Lindenbaum T (i+1)} : (∏l)ᶜ = ∐lᶜ :=
+lemma prenex_fal_neg {l : Lindenbaum T (i+1)} : (∏ l)ᶜ = ∐ lᶜ :=
 by { have := prenex_ex_neg lᶜ, simp at this, simp[←this] }
 
 lemma prenex_fal_or_left {l : Lindenbaum T (i+1)} {k : Lindenbaum T i} :
-  ∏l ⊔ k = ∏(l ⊔ sf k) :=
+  ∏ l ⊔ k = ∏ (l ⊔ sf k) :=
 begin
   induction l using fopl.Lindenbaum.ind_on, induction k using fopl.Lindenbaum.ind_on,
   simp[fal, has_sup.sup, sf, Lindenbaum.of_eq_of, formula.or], split,
   { refine (deduction.mp $ GE $ contrapose.mp _), rw [←sf_dsb], simp,
-    have lmm₁ : ⇑(T ^ i)+{¬̇(∀̇l).sf →̇ k.sf} ⊢̇ ¬̇k.sf →̇ (∀̇l).sf, { apply contrapose.mp, simp },
-    have lmm₂ : ⇑(T ^ i)+{¬̇(∀̇l).sf →̇ k.sf} ⊢̇ (∀̇l).sf →̇ l,
-    { suffices : ⇑(T ^ i)+{¬̇(∀̇l).sf →̇ k.sf} ⊢̇ (∀̇l).sf →̇ (l.rew $ shift^1).rew ₛ[#0],
+    have lmm₁ : ⇑(T^i)+{¬̇(∀̇ l).sf →̇ k.sf} ⊢ ¬̇k.sf →̇ (∀̇ l).sf, { apply contrapose.mp, simp },
+    have lmm₂ : ⇑(T^i)+{¬̇(∀̇ l).sf →̇ k.sf} ⊢ (∀̇ l).sf →̇ l,
+    { suffices : ⇑(T^i)+{¬̇(∀̇ l).sf →̇ k.sf} ⊢ (∀̇ l).sf →̇ (l.rew $ shift^1).rew ₛ[#0],
       { simp* at* },
       exact provable.q1 },
     exact lmm₁.imp_trans lmm₂ },
   { refine (deduction.mp $ contrapose.mp $ deduction.mp _), simp,
     refine GE _, simp[←sf_dsb], refine deduction.mpr _,
-    show ⇑(T ^ i)+{(∀̇(¬̇l →̇ k.sf)).sf} ⊢̇ ¬̇k.sf →̇ l,
-    have : ⇑(T ^ i)+{(∀̇(¬̇l →̇ k.sf)).sf} ⊢̇ ¬̇l →̇ k.sf,
-    { have : ⇑(T ^ i)+{(∀̇(¬̇l →̇ k.sf)).sf} ⊢̇ (∀̇(¬̇l →̇ k.sf)).sf, { simp },
+    show ⇑(T^i)+{(∀̇  (¬̇l →̇ k.sf)).sf} ⊢ ¬̇k.sf →̇ l,
+    have : ⇑(T^i)+{(∀̇  (¬̇l →̇ k.sf)).sf} ⊢ ¬̇l →̇ k.sf,
+    { have : ⇑(T^i)+{(∀̇  (¬̇l →̇ k.sf)).sf} ⊢ (∀̇  (¬̇l →̇ k.sf)).sf, { simp },
       have lmm₁ := this.fal_subst #0, simp at lmm₁,
       exact lmm₁ },
     apply contrapose.mp, simp[this] }
 end
 
 lemma prenex_fal_or_right {l : Lindenbaum T i} {k : Lindenbaum T (i+1)} :
-  l ⊔ ∏k = ∏(sf l ⊔ k) :=
-by simp[show l ⊔ ∏k = ∏k ⊔ l, from sup_comm, prenex_fal_or_left,
+  l ⊔ ∏ k = ∏ (sf l ⊔ k) :=
+by simp[show l ⊔ ∏ k = ∏ k ⊔ l, from sup_comm, prenex_fal_or_left,
         show k ⊔ l.sf = l.sf ⊔ k, from sup_comm]
 
 lemma prenex_fal_and_left {l : Lindenbaum T (i+1)} {k : Lindenbaum T i} :
-  ∏l ⊓ k = ∏(l ⊓ sf k) :=
+  ∏ l ⊓ k = ∏ (l ⊓ sf k) :=
 begin
   induction l using fopl.Lindenbaum.ind_on, induction k using fopl.Lindenbaum.ind_on,
   simp[fal, has_inf.inf, sf, Lindenbaum.of_eq_of], split,
   { refine (deduction.mp $ GE _), rw [←sf_dsb], simp[axiom_and],
-    have : ⇑(T ^ i)+{(∀̇l).sf}+{k.sf} ⊢̇ (∀̇l).sf, simp,
+    have : ⇑(T^i)+{(∀̇ l).sf}+{k.sf} ⊢ (∀̇ l).sf, simp,
     have := this.fal_subst #0, simp* at* },
   { refine deduction.mp _, simp,
      split,
     { refine GE _, simp[←sf_dsb],
-      have : ⇑(T ^ i)+{(∀̇(l ⩑ k.sf)).sf} ⊢̇ (∀̇(l ⩑ k.sf)).sf, simp,
+      have : ⇑(T^i)+{(∀̇  (l ⩑ k.sf)).sf} ⊢ (∀̇  (l ⩑ k.sf)).sf, simp,
       have := this.fal_subst #0, simp* at* },
-    { have : (T ^ i)+{∀̇(l ⩑ k.sf)} ⊢̇ ∀̇(l ⩑ k.sf), simp,
+    { have : (T^i)+{∀̇  (l ⩑ k.sf)} ⊢ ∀̇  (l ⩑ k.sf), simp,
       have := this.fal_subst #0, simp* at * } }
 end
 
 lemma prenex_ex_or_left {l : Lindenbaum T (i+1)} {k : Lindenbaum T i} :
-  ∐l ⊔ k = ∐(l ⊔ sf k) :=
+  ∐ l ⊔ k = ∐ (l ⊔ sf k) :=
 begin
   rw ← compl_inj_iff, simp[-compl_inj_iff, prenex_ex_neg, prenex_fal_and_left],
 end
@@ -638,21 +635,21 @@ by { induction l using fopl.Lindenbaum.ind_on,
      induction m using fopl.Lindenbaum.ind_on,
      simp[has_le.le, has_top.top, has_compl.compl, has_sup.sup, Lindenbaum.of_eq_of, formula.or] }
 
-@[simp] lemma fal_top_top : (∏⊤ : Lindenbaum T i) = ⊤ :=
+@[simp] lemma fal_top_top : (∏ ⊤ : Lindenbaum T i) = ⊤ :=
 by { simp[has_top.top, fal, Lindenbaum.of_eq_of], apply provable.GE, simp }
 
-@[simp] lemma ex_top_top : (∐⊤ : Lindenbaum T i) = ⊤ :=
+@[simp] lemma ex_top_top : (∐ ⊤ : Lindenbaum T i) = ⊤ :=
 by { simp[has_top.top, ex, Lindenbaum.of_eq_of], apply provable.use #0, simp }
 
-theorem provable_top_iff {p} : T^i ⊢̇ p ↔ (⟦p⟧ᴸ : Lindenbaum T i) = ⊤ := by simp[has_top.top, Lindenbaum.of_eq_of]
+theorem provable_top_iff {p} : T^i ⊢ p ↔ (⟦p⟧ᴸ : Lindenbaum T i) = ⊤ := by simp[has_top.top, Lindenbaum.of_eq_of]
 
-protected theorem provable_iff {p q} : T^i ⊢̇ p ↔̇ q ↔ (⟦p⟧ᴸ : Lindenbaum T i) = ⟦q⟧ᴸ :=
+protected theorem provable_iff {p q} : T^i ⊢ p ↔̇ q ↔ (⟦p⟧ᴸ : Lindenbaum T i) = ⟦q⟧ᴸ :=
 by simp[Lindenbaum.of_eq_of]
 
-protected theorem provable_iff0 {p q} : T ⊢̇ p ↔̇ q ↔ (⟦p⟧ᴸ : Lindenbaum T 0) = ⟦q⟧ᴸ :=
+protected theorem provable_iff0 {p q} : T ⊢ p ↔̇ q ↔ (⟦p⟧ᴸ : Lindenbaum T 0) = ⟦q⟧ᴸ :=
 by simp[Lindenbaum.of_eq_of]
 
-theorem provable_imp_iff {p q} : T^i ⊢̇ p →̇ q ↔ (⟦p⟧ᴸ : Lindenbaum T i) ≤ ⟦q⟧ᴸ := by simp[has_le.le]
+theorem provable_imp_iff {p q} : T^i ⊢ p →̇ q ↔ (⟦p⟧ᴸ : Lindenbaum T i) ≤ ⟦q⟧ᴸ := by simp[has_le.le]
 
 @[simp] lemma provable_top_eq : (⟦⊤̇⟧ᴸ : Lindenbaum T i) = ⊤ := rfl
 @[simp] lemma provable_bot_eq : (⟦⊥̇⟧ᴸ : Lindenbaum T i) = ⊥ := rfl
@@ -662,7 +659,7 @@ theorem provable_imp_iff {p q} : T^i ⊢̇ p →̇ q ↔ (⟦p⟧ᴸ : Lindenbau
 @[simp] theorem provable_imp_eq {p q} : (⟦p →̇ q⟧ᴸ : Lindenbaum T i) = ⟦p⟧ᴸᶜ ⊔ ⟦q⟧ᴸ := by {
   have : (⟦p →̇ q⟧ᴸ : Lindenbaum T i) = ⟦¬̇p ⩒ q⟧ᴸ, 
   { simp[Lindenbaum.of_eq_of, -provable_or_eq, formula.or], refine ⟨deduction.mp (by simp), deduction.mp _⟩,
-    have : (T^i)+{¬̇¬̇p →̇ q} ⊢̇ ¬̇¬̇p →̇ q, simp[-dn1_iff], simp* at* },
+    have : (T^i)+{¬̇¬̇p →̇ q} ⊢ ¬̇¬̇p →̇ q, simp[-dn1_iff], simp* at* },
   simp[this] }
 
 @[simp] lemma provable_equal_eq {t₁ t₂} : (⟦t₁ =̇ t₂⟧ᴸ : Lindenbaum T i) = ⟦t₁⟧ᴴ ∥ ⟦t₂⟧ᴴ := rfl
@@ -670,15 +667,15 @@ theorem provable_imp_iff {p q} : T^i ⊢̇ p →̇ q ↔ (⟦p⟧ᴸ : Lindenbau
 @[simp] theorem provable_predicate₂_iff {p : L.pr 2} {t₁ t₂} :
   (⟦formula.app p (vecterm.cons t₁ t₂)⟧ᴸ : Lindenbaum T i) = predicate₂ T i p ⟦t₁⟧ᴴ ⟦t₂⟧ᴴ := rfl 
 
-@[simp] theorem provable_fal_eq {p} : (⟦∀̇p⟧ᴸ : Lindenbaum T i) = ∏⟦p⟧ᴸ := rfl
-@[simp] theorem provable_ex_eq {p} : (⟦∃̇p⟧ᴸ : Lindenbaum T i) = ∐⟦p⟧ᴸ := rfl
+@[simp] theorem provable_fal_eq {p} : (⟦∀̇ p⟧ᴸ : Lindenbaum T i) = ∏  ⟦p⟧ᴸ := rfl
+@[simp] theorem provable_ex_eq {p} : (⟦∃̇ p⟧ᴸ : Lindenbaum T i) = ∐  ⟦p⟧ᴸ := rfl
 
 lemma to_Herbrand {h₁ h₂ : Herbrand T i} : h₁ ∥ h₂ = ⊤ ↔ h₁ = h₂ :=
 by { induction h₁ using fopl.Herbrand.ind_on, induction h₂ using fopl.Herbrand.ind_on,
      simp only [equal, Herbrand.of_eq_of, has_top.top],
      simp[-provable_equal_eq, -provable_top_eq, Lindenbaum.of_eq_of] }
 
-theorem provable_neg_iff {p} : T^i ⊢̇ ¬̇p ↔ (⟦p⟧ᴸ : Lindenbaum T i) = ⊥ :=
+theorem provable_neg_iff {p} : T^i ⊢ ¬̇p ↔ (⟦p⟧ᴸ : Lindenbaum T i) = ⊥ :=
 by simp[provable_top_iff]
 
 end Lindenbaum
