src/deduction.lean
@@ -1,25 +1,9 @@
-import fopl
+import fopl theory
 
 universe u
 
 namespace fopl
 variables {L : language.{u}}
-
-def theory (L : language) := set (formula L)
-
-notation `theory `L:max := set (formula L)
-
-inductive theory.sf (T : theory L) : theory L
-| intro : ∀ {p : formula L}, p ∈ T → theory.sf p.sf
-prefix `⇑`:max := theory.sf
-
-@[simp, reducible] def theory.sf_itr (T : theory L) : ℕ → theory L
-| 0     := T
-| (n+1) := ⇑(theory.sf_itr n)
-instance sf_itr_pow : has_pow (theory L) ℕ := ⟨theory.sf_itr⟩
-
-@[simp] lemma sf_itr_0 (T : theory L) : T^0 = T := rfl
-@[simp] lemma sf_itr_succ (T : theory L) (n) : T^(n+1) = ⇑(T^n) := rfl
 
 @[simp] def formula.equals : ∀ {n}, vecterm L n → vecterm L n → formula L
 | 0     t₁                   t₂                   := t₁ =̇ t₂
@@ -32,15 +16,15 @@ infix ` ≡̇ `:90 := formula.equals
     by simp[formula.rew, vecterm.rew, equals_rew v₁ v₂]
 
 inductive provable : theory L → formula L → Prop
-| GE : ∀ {T : theory L} {p}, provable ⇑T p → provable T (∀̇p)
+| GE : ∀ {T : theory L} {p}, provable ⇑T p → provable T (∀̇ p)
 | MP : ∀ {T : theory L} {p q}, provable T (p →̇ q) → provable T p → provable T q
 | AX : ∀ {T : theory L} {p}, p ∈ T → provable T p
 | p1 : ∀ {T : theory L} {p q}, provable T (p →̇ q →̇ p)
 | p2 : ∀ {T : theory L} {p q r}, provable T ((p →̇ q →̇ r) →̇ (p →̇ q) →̇ p →̇ r)
 | p3 : ∀ {T : theory L} {p q}, provable T ((¬̇p →̇ ¬̇q) →̇ q →̇ p)
-| q1 : ∀ {T : theory L} {p t}, provable T (∀̇p →̇ p.rew ₛ[t])
-| q2 : ∀ {T : theory L} {p q}, provable T (∀̇(p →̇ q) →̇ ∀̇p →̇∀̇q)
-| q3 : ∀ {T : theory L} {p}, provable T (p →̇ ∀̇p.sf)
+| q1 : ∀ {T : theory L} {p t}, provable T (∀̇ p →̇ p.rew ₛ[t])
+| q2 : ∀ {T : theory L} {p q}, provable T (∀̇ (p →̇ q) →̇ ∀̇ p →̇∀̇ q)
+| q3 : ∀ {T : theory L} {p}, provable T (p →̇ ∀̇ p.sf)
 | e1 : ∀ {T : theory L} {t}, provable T (t =̇ t)
 | e2 : ∀ {T : theory L} {t₁ t₂}, provable T (t₁ =̇ t₂ →̇ t₂ =̇ t₁)
 | e3 : ∀ {T : theory L} {t₁ t₂ t₃}, provable T (t₁ =̇ t₂ →̇ t₂ =̇ t₃ →̇ t₁ =̇ t₃)
@@ -49,146 +33,18 @@ inductive provable : theory L → formula L → Prop
 | e5 : ∀ {T : theory L} {n} {v₁ v₂ : vecterm L n} {r : L.pr (n+1)},
     provable T (v₁ ≡̇ v₂ →̇ formula.app r v₁ →̇ formula.app r v₂)
 
-infix ` ⊢̇ `:60 := provable
+infix ` ⊢ `:60 := provable
 
 attribute [simp] provable.p1 provable.p2 provable.p3 provable.q1 provable.q2 provable.q3
   provable.e1 provable.e2 provable.e3 provable.e4 provable.e5
 
-def theory.consistent (T : theory L) : Prop := ¬∃p, (T ⊢̇ p) ∧ (T ⊢̇ ¬̇p) 
+def theory.consistent (T : theory L) : Prop := ¬∃p, (T ⊢ p) ∧ (T ⊢ ¬̇p) 
 
-inductive theory.add (T : theory L) (p : formula L) : theory L 
-| new : theory.add p
-| old : ∀ {q}, q ∈ T → theory.add q
-
-notation T`+{`:max p`}` := theory.add T p
-
-def theory.le (T U : theory L) : Prop := ∀ p, T ⊢̇ p → U ⊢̇ p
+def theory.le (T U : theory L) : Prop := ∀ p, T ⊢ p → U ⊢ p
 
 instance : has_le (theory L) := ⟨theory.le⟩
 
-class closed_theory (T : theory L) := (cl : ∀ {p}, p ∈ T → sentence p)
-
-class extend (T₀ T : theory L) := (ss : T₀ ⊆ T)
-
-def proper_at (n : ℕ) (T : theory L) : Prop := ∀ (p : formula L) (s), p ∈ T → p.rew (s^n) ∈ T
-
-def ordered_p (T : theory L) : Prop := ∀ (p : formula L), p ∈ T → p.sf ∈ T
-
-class ordered (T : theory L) := (ordered : ordered_p T)
-
-lemma oedered_p_theory_sf (T : theory L) : ordered_p T → ordered_p ⇑T := λ h p hyp,
-by { cases hyp with p hyp_p, exact theory.sf.intro (h _ hyp_p) }
-
-instance ordered_theory_sf {T : theory L} [od : ordered T] :
-  ordered ⇑T := ⟨oedered_p_theory_sf _ od.ordered⟩
-
-instance ordered_theory_sf_itr {T : theory L} [od : ordered T] : ∀ n : ℕ, ordered (T^n)
-| 0 := od
-| (n+1) := @fopl.ordered_theory_sf _ _  (ordered_theory_sf_itr n)
-
-class proper (n : ℕ) (T : theory L) := (proper : proper_at n T)
-
-instance ordered_proper {T : theory L} [pp : proper 0 T] : ordered T :=
-⟨λ p h, by { have := pp.proper, exact this _ (λ x, #(x+1)) h }⟩
-
-lemma proper.proper0 {T : theory L} [proper 0 T] :
-  ∀ {p : formula L} {s}, p ∈ T → p.rew s ∈ T := @proper.proper _ 0 T _
-
-instance : closed_theory (∅ : theory L) := ⟨λ _ h, by exfalso; exact h⟩
-
-instance (n) : proper n (∅ : theory L) := ⟨λ _ _ h, by exfalso; exact h⟩
-
-instance (n) : proper n (set.univ : theory L) := ⟨λ p s h, by simp⟩
-
-def openform : theory L := {p | p.Open = tt}
-
-instance (n) : proper n (openform : theory L) :=
-⟨λ p s h, by { induction p; simp[openform] at*; simp* at* }⟩
-
-lemma theory_sf_itr_sf_itr {T : theory L} : ∀ {n} {p : formula L},
-  p ∈ T^n → ∃ q : formula L, p = (q.rew (λ x, #(x+n))) ∧ q ∈ T
-| 0 p h := by { simp, exact h }
-| (n+1) p h := by { simp at h, cases h with p' hyp_p',
-    have IH := theory_sf_itr_sf_itr hyp_p', rcases IH with ⟨q, hyp_q⟩,
-    refine ⟨q, _⟩,
-    have : q.rew (λ x, #(x + (n + 1))) = (q.rew (λ x, #(x + n))).sf,
-    { simp[formula.sf, formula.nested_rew, add_assoc] }, simp[this, hyp_q], refl }
-
-lemma mem_theory_sf_itr {T : theory L} : ∀ (n) {p : formula L},
-  p ∈ T → p.sf_itr n ∈ T^n
-| 0     p h := by simp[has_pow.pow, formula.sf_itr, h]
-| (n+1) p h := by { simp[formula.sf_itr],
-    have lmm₁ : (p.sf_itr n).sf ∈ ⇑(T^n) := theory.sf.intro (@mem_theory_sf_itr n _ h),
-    have : p.rew (λ x, #(x + (n + 1))) = (p.sf_itr n).sf,
-    { simp[formula.sf, formula.sf_itr, formula.nested_rew, add_assoc] },
-    simp[this], exact lmm₁ }
-
-lemma sentence_mem_theory_sf_itr {T : theory L} {p : formula L} (a : sentence p) (n : ℕ) :
-  p ∈ T → p ∈ T^n := λ h,
-by { have : p.rew (λ x, #(x+n)) = p, exact formula.sentence_rew a _, rw ←this,
-     refine mem_theory_sf_itr _ h }
-
-lemma proper_sf_inclusion (T : theory L) [proper 0 T] : ∀ {n m : ℕ} (h : n ≤ m),
-  T^m ⊆ T^n :=
-begin
-  suffices : ∀ {n m : ℕ}, T^(n+m) ⊆ T^n,
-  { intros n m eqn p hyp, have e : m = n + (m - n), exact (nat.add_sub_of_le eqn).symm, 
-    rw e at hyp,
-    exact this hyp },
-  intros n m p h,
-  induction m with m IH, { exact h },
-  { suffices : p ∈ T^(n + m), from IH this,
-    have := theory_sf_itr_sf_itr h, rcases this with ⟨q, rfl, lmm⟩,
-    have : q.sf ∈ T, { simp[formula.sf, proper.proper0 lmm] },
-    have : q.sf.sf_itr (n + m) ∈ T^(n+m), from mem_theory_sf_itr _ this,
-    have eqn : q.rew (λ x, #(x + n + m + 1)) = q.sf.sf_itr (n + m),
-    { simp[formula.sf, formula.sf_itr, formula.nested_rew, nat.succ_add_eq_succ_add, ←add_assoc],refl },
-    simp[←nat.add_one m, ←add_assoc, eqn] at ⊢, exact this }
-end
-
-lemma ordered_inclusion (T : theory L) [ordered T] : ⇑T ⊆ T := λ p h,
-by { cases h with p hyp, exact ordered.ordered _ hyp }
-
-lemma formula.sf_rew_sf_eq (s) (p : formula L) : p.sf.rew (s^1) = (p.rew s).sf :=
-by { simp[formula.sf, formula.nested_rew] }
-
-lemma proper_theory_sf {n : ℕ} {T : theory L} (pp : proper_at n T) :
-  proper_at (n+1) ⇑T := λ p s h,
-by { cases h with p hyp_p,
-     show p.sf.rew ((s^n)^1) ∈ ⇑T, simp[formula.sf_rew_sf_eq],
-     refine theory.sf.intro (pp _ _ hyp_p) }
-
-instance properc_theory_sf {n : ℕ} {T : theory L} [pp : proper n T] :
-  proper (n+1) (⇑T) := ⟨
-by { have : proper_at n T, from @proper.proper L n T pp,
-     have : proper_at (n+1) ⇑T, from proper_theory_sf this, exact this }⟩
-
-lemma proper_theory_sf_itr {n : ℕ} {T : theory L} (pp : proper_at n T) : ∀ m,
-  proper_at (n+m) (T^m)
-| 0     := by { simp, exact @pp }
-| (m+1) := by { simp[←add_assoc], exact proper_theory_sf (proper_theory_sf_itr m) }
-
-instance properc_theory_sf_itr {T : theory L} [pp : proper 0 T] {n} :
-  proper n (T^n) := ⟨by { have := proper_theory_sf_itr pp.proper n, simp* at* }⟩ 
-
-lemma closed_proper {T : theory L} [cl : closed_theory T] : proper_at 0 T :=
-λ p s h, by { simp[@closed_theory.cl _ _ cl _ h], exact h }
-
-@[simp] lemma closed_theory_sf_eq {T : theory L} [cl : closed_theory T] : ⇑T = T :=
-by { ext p, refine ⟨λ hyp, _, λ hyp, _⟩, cases hyp with p hyp_p,
-     simp[formula.sentence_rew (closed_theory.cl hyp_p), hyp_p],
-     rw ← (formula.sentence_sf (closed_theory.cl hyp)), refine theory.sf.intro hyp }
-
-lemma sf_dsb (T : theory L) (p : formula L) : ⇑T+{p.sf} = ⇑(T+{p}) :=
-begin
-  ext x, split; intros h,
-  { cases h with h hx, refine theory.sf.intro theory.add.new,
-    cases hx with p hp, refine theory.sf.intro (theory.add.old hp) },
-  { cases h with q hq, cases hq with _ hq, refine theory.add.new,
-    refine theory.add.old (theory.sf.intro hq) }
-end
-
-def theory.th (T : theory L) : theory L := {p | T ⊢̇ p}
+def theory.th (T : theory L) : theory L := {p | T ⊢ p}
 
 def conjunction : list (formula L) → formula L
 | []        := ⊤̇
@@ -200,41 +56,41 @@ by { intros s₁, suffices : ∀ t, U s₁ ⊆ U (s₁ + t),
         rw (show s₁ + (s₂ - s₁) = s₂, from nat.add_sub_of_le eqn) at this, exact this },
       intros t, induction t with t IH, simp, rw[nat.add_succ],  refine λ x hx, hyp _ (IH hx) }
 
-def formula.equiv (T : theory L) (p₁ p₂ : formula L) : Prop := T ⊢̇ p₁ ↔̇ p₂
+def formula.equiv (T : theory L) (p₁ p₂ : formula L) : Prop := T ⊢ p₁ ↔̇ p₂
 
-def term.equiv (T : theory L) (t₁ t₂ : term L) : Prop := T ⊢̇ t₁ =̇ t₂
+def term.equiv (T : theory L) (t₁ t₂ : term L) : Prop := T ⊢ t₁ =̇ t₂
 
 namespace provable
 variables (T : theory L)
 
-@[simp] lemma pp (p) : T ⊢̇ p →̇ p :=
+@[simp] lemma pp (p) : T ⊢ p →̇ p :=
 begin
-  have l₀ : T ⊢̇ (p →̇ (p →̇ p) →̇ p) →̇ (p →̇ p →̇ p) →̇ p →̇ p, simp,
-  have l₁ : T ⊢̇ p →̇ (p →̇ p) →̇ p, simp,
-  have l₂ : T ⊢̇ (p →̇ p →̇ p) →̇ p →̇ p, refine l₀.MP l₁,
-  have l₃ : T ⊢̇ p →̇ p →̇ p, simp,
+  have l₀ : T ⊢ (p →̇ (p →̇ p) →̇ p) →̇ (p →̇ p →̇ p) →̇ p →̇ p, simp,
+  have l₁ : T ⊢ p →̇ (p →̇ p) →̇ p, simp,
+  have l₂ : T ⊢ (p →̇ p →̇ p) →̇ p →̇ p, refine l₀.MP l₁,
+  have l₃ : T ⊢ p →̇ p →̇ p, simp,
   refine l₂.MP l₃
 end
 
-@[simp] lemma top : T ⊢̇ ⊤̇ := by simp[formula.top]; exact GE (by simp)
+@[simp] lemma top : T ⊢ ⊤̇ := by simp[formula.top]; exact GE (by simp)
 
-@[simp] lemma add (p) : T+{p} ⊢̇ p :=
+@[simp] lemma add (p) : T+{p} ⊢ p :=
 AX (theory.add.new)
 
 variables {T}
 
-lemma GE_cl {T : theory L} [closed_theory T] {p} (h : T ⊢̇ p) : T ⊢̇ ∀̇p :=
+lemma GE_cl {T : theory L} [closed_theory T] {p} (h : T ⊢ p) : T ⊢ ∀̇p :=
 by { apply provable.GE, simp[h] }
 
-@[simp] lemma imp_r {p} (h : T ⊢̇ p) (q) : T ⊢̇ q →̇ p :=
-by { have : T ⊢̇ p →̇ q →̇ p, simp,
+@[simp] lemma imp_r {p} (h : T ⊢ p) (q) : T ⊢ q →̇ p :=
+by { have : T ⊢ p →̇ q →̇ p, simp,
      exact this.MP h }
 
-lemma imp_trans {p q r} : (T ⊢̇ p →̇ q) → (T ⊢̇ q →̇ r) → (T ⊢̇ p →̇ r) := λ h₁ h₂,
+lemma imp_trans {p q r} : (T ⊢ p →̇ q) → (T ⊢ q →̇ r) → (T ⊢ p →̇ r) := λ h₁ h₂,
 begin
-  have l₁ : T ⊢̇ (p →̇ q →̇ r) →̇ (p →̇ q) →̇ (p →̇ r), simp,  
-  have l₂ : T ⊢̇ (p →̇ q →̇ r), simp[h₂],
-  have l₃ : T ⊢̇ (p →̇ q) →̇ (p →̇ r), from l₁.MP l₂,
+  have l₁ : T ⊢ (p →̇ q →̇ r) →̇ (p →̇ q) →̇ (p →̇ r), simp,  
+  have l₂ : T ⊢ (p →̇ q →̇ r), simp[h₂],
+  have l₃ : T ⊢ (p →̇ q) →̇ (p →̇ r), from l₁.MP l₂,
   exact l₃.MP h₁
 end
 
@@ -242,15 +98,15 @@ lemma nfal_eq : ∀ (n) (p : formula L), nfal (∀̇p) n = ∀̇(nfal (p) n)
 | 0     p := rfl
 | (n+1) p := by simp; exact nfal_eq n p
 
-lemma GE_itr : ∀ {n p}, T^n ⊢̇ p → T ⊢̇ nfal p n
+lemma GE_itr : ∀ {n p}, T^n ⊢ p → T ⊢ nfal p n
 | 0     p h := by simp* at*
 | (n+1) p h := by { simp[←nfal_eq] at*, exact GE_itr (GE h) }
 
 lemma subst_itr : ∀ (n) (p : formula L) (s : ℕ → term L),
-  T ⊢̇ nfal p n →̇ p.rew (λ x, if x < n then s x else #(x-n))
+  T ⊢ nfal p n →̇ p.rew (λ x, if x < n then s x else #(x-n))
 | 0 p s := by simp
 | (n+1) p s := by { simp,
-    have lmm₁ : T ⊢̇ ∀̇(nfal p n) →̇ nfal (p.rew $ ₛ[s n]^n) n,
+    have lmm₁ : T ⊢ ∀̇(nfal p n) →̇ nfal (p.rew $ ₛ[s n]^n) n,
     { have := @provable.q1 _ T (nfal p n) (s n), simp[formula.nfal_rew] at this,
       have eqn : (λ m, ite (m < n) #m ((ₛ[s n] (m - n)).rew (λ x, #(x+n)))) = ₛ[s n]^n,
       { ext m,
@@ -277,54 +133,54 @@ lemma subst_itr : ∀ (n) (p : formula L) (s : ℕ → term L),
     simp[this] at lmm₂,
     exact lmm₁.imp_trans lmm₂ }
 
-lemma inclusion {p} (h : T ⊢̇ p) : ∀ {U}, T ⊆ U → U ⊢̇ p :=
+lemma inclusion {p} (h : T ⊢ p) : ∀ {U}, T ⊆ U → U ⊢ p :=
 begin
   induction h with T p hyp_p IH T p q hyp_pq hyp_p IH₁ IH₂ T p hyp_p; try { simp },
-  { intros U hyp, refine GE (IH (λ x h, _)), cases h with p hp,
-    refine theory.sf.intro _, exact hyp hp },
+  { intros U hyp, refine GE (IH (λ x h, _)), rcases h with ⟨p, hp, rfl⟩,
+    refine ⟨p, hyp hp, rfl⟩ },
   { intros U hyp, exact (IH₁ hyp).MP (IH₂ hyp) },
   { intros U hyp, exact AX (hyp hyp_p) }
 end
 
-@[simp] lemma weakening {q} (h : T ⊢̇ q) (p) : T+{p} ⊢̇ q :=
+@[simp] lemma weakening {q} (h : T ⊢ q) (p) : T+{p} ⊢ q :=
 inclusion h (λ x h, theory.add.old h)
 
-private lemma delete_imply {p} (h : T ⊢̇ p) : ∀ q, T \ {q} ⊢̇ q →̇ p :=
+private lemma delete_imply {p} (h : T ⊢ p) : ∀ q, T \ {q} ⊢ q →̇ p :=
 begin
   induction h with T p hyp_p IH T p₁ p₂ hyp_p₁₂ hyp_p₁ IH₁ IH₂ T p hyp_p;
     try { intros q, apply imp_r, simp }; intros q,
-  { have IH : ⇑T \ {q.sf} ⊢̇ q.sf →̇ p := IH q.sf,
-    have lmm₁ : T \ {q} ⊢̇ q →̇ ∀̇ q.sf, { simp },
-    have lmm₂ : T \ {q} ⊢̇ ∀̇ q.sf →̇ ∀̇ p,
-    { suffices : T \ {q} ⊢̇ ∀̇(q.sf →̇ p),
-      { have lmm : T \ {q} ⊢̇ ∀̇(q.sf →̇ p) →̇ ∀̇ q.sf →̇ ∀̇ p, simp,
+  { have IH : ⇑T \ {q.sf} ⊢ q.sf →̇ p := IH q.sf,
+    have lmm₁ : T \ {q} ⊢ q →̇ ∀̇ q.sf, { simp },
+    have lmm₂ : T \ {q} ⊢ ∀̇ q.sf →̇ ∀̇ p,
+    { suffices : T \ {q} ⊢ ∀̇(q.sf →̇ p),
+      { have lmm : T \ {q} ⊢ ∀̇(q.sf →̇ p) →̇ ∀̇ q.sf →̇ ∀̇ p, simp,
         exact lmm.MP this },
       refine GE (inclusion IH (λ x h, _)), 
-      rcases h with ⟨h, neq⟩, rcases h with ⟨p', h'⟩,
-      refine theory.sf.intro ⟨h', λ c, _⟩, simp at c,
+      rcases h with ⟨h, neq⟩, rcases h with ⟨p', h', rfl⟩,
+      refine ⟨p', ⟨h', λ c, _⟩, rfl⟩, simp at c,
       rw c at neq, exact neq rfl },
     exact lmm₁.imp_trans lmm₂ },
-  { have : T \ {q} ⊢̇ (q →̇ p₁ →̇ p₂) →̇ (q →̇ p₁) →̇ (q →̇ p₂), simp, 
-    have : T \ {q} ⊢̇ (q →̇ p₁) →̇ q →̇ p₂, from this.MP (IH₁ _),
+  { have : T \ {q} ⊢ (q →̇ p₁ →̇ p₂) →̇ (q →̇ p₁) →̇ (q →̇ p₂), simp, 
+    have : T \ {q} ⊢ (q →̇ p₁) →̇ q →̇ p₂, from this.MP (IH₁ _),
     exact this.MP (IH₂ _) },
   { by_cases eqn : p = q,
     { simp[eqn] },
-    { have : T \ {q} ⊢̇ p, from AX ⟨hyp_p, eqn⟩,
+    { have : T \ {q} ⊢ p, from AX ⟨hyp_p, eqn⟩,
       simp[this] } }
 end
 
-theorem deduction {p q} : (T+{p} ⊢̇ q) ↔ (T ⊢̇ p →̇ q) :=
-⟨λ h, by { have : (T+{p}) \ {p} ⊢̇ p →̇ q, from delete_imply h p,
+theorem deduction {p q} : (T+{p} ⊢ q) ↔ (T ⊢ p →̇ q) :=
+⟨λ h, by { have : (T+{p}) \ {p} ⊢ p →̇ q, from delete_imply h p,
            refine inclusion this (λ x h, _), rcases h with ⟨h, neq⟩,
            cases h; simp* at*, },
- λ h, by { have : T+{p} ⊢̇ p →̇ q, from weakening h p,
+ λ h, by { have : T+{p} ⊢ p →̇ q, from weakening h p,
            exact this.MP (by simp) }⟩
 
 theorem proof_compact : ∀ {T : ℕ → theory L}, (∀ s, T s ⊆ T (s+1)) →
-  ∀ {p}, {p | ∃ s, T s p} ⊢̇ p → ∃ s, T s ⊢̇ p :=
+  ∀ {p}, {p | ∃ s, T s p} ⊢ p → ∃ s, T s ⊢ p :=
 begin
-  suffices : ∀ {p} {U : theory L}, U ⊢̇ p → ∀ {T : ℕ → theory L},
-    (∀ s, T s ⊆ T (s+1)) → U ⊆ {p | ∃ s, T s p} → ∃ s, T s ⊢̇ p,
+  suffices : ∀ {p} {U : theory L}, U ⊢ p → ∀ {T : ℕ → theory L},
+    (∀ s, T s ⊆ T (s+1)) → U ⊆ {p | ∃ s, T s p} → ∃ s, T s ⊢ p,
   { refine λ T hyp p h, this h hyp (λ x hx, hx) },
   intros p U h,
   induction h,
@@ -332,19 +188,20 @@ begin
   { intros U hyp ss,
     let U' := λ s, ⇑(U s),
     have hyp' : ∀ s, U' s ⊆ U' (s + 1),
-    { simp[U'], intros s p hyp_p, cases hyp_p with p' hyp_q', refine theory.sf.intro (hyp _ hyp_q') },
+    { simp[U'], intros s p hyp_p, rcases hyp_p with ⟨p', hyp_q', rfl⟩,
+      refine ⟨p', hyp _ hyp_q', rfl⟩ },
     have ss' : ⇑T ⊆ {p : formula L | ∃ s, U' s p},
-    { intros q hyp_q, cases hyp_q with q' hyp_q', rcases (ss hyp_q') with ⟨s, hyp_s⟩,
-      refine ⟨s, theory.sf.intro hyp_s⟩ },
-    have : ∃ s, U' s ⊢̇ p, from IH hyp' ss', rcases this with ⟨s, h⟩,
+    { intros q hyp_q, rcases hyp_q with ⟨q', hyp_q', rfl⟩, rcases (ss hyp_q') with ⟨s, hyp_s⟩,
+      refine ⟨s, _, hyp_s, rfl⟩ },
+    have : ∃ s, U' s ⊢ p, from IH hyp' ss', rcases this with ⟨s, h⟩,
     refine ⟨s, provable.GE h⟩ },
   case fopl.provable.MP : T p q hyp_pq hyp_p IH₁ IH₂
   { intros U hyp ss,
-    have : ∃ s, U s ⊢̇ p →̇ q, from IH₁ hyp ss, rcases this with ⟨s₁, lmm₁⟩,
-    have : ∃ s, U s ⊢̇ p, from IH₂ hyp ss, rcases this with ⟨s₂, lmm₂⟩,
+    have : ∃ s, U s ⊢ p →̇ q, from IH₁ hyp ss, rcases this with ⟨s₁, lmm₁⟩,
+    have : ∃ s, U s ⊢ p, from IH₂ hyp ss, rcases this with ⟨s₂, lmm₂⟩,
     refine ⟨max s₁ s₂, _⟩,
-    have lmm₁ : U (max s₁ s₂) ⊢̇ p →̇ q, from provable.inclusion lmm₁ (ss_le hyp (by simp)),
-    have lmm₂ : U (max s₁ s₂) ⊢̇ p, from provable.inclusion lmm₂ (ss_le hyp (by simp)),
+    have lmm₁ : U (max s₁ s₂) ⊢ p →̇ q, from provable.inclusion lmm₁ (ss_le hyp (by simp)),
+    have lmm₂ : U (max s₁ s₂) ⊢ p, from provable.inclusion lmm₂ (ss_le hyp (by simp)),
     exact lmm₁.MP lmm₂ },
   case fopl.provable.AX : T p hyp_p
   { intros U hyp ss, rcases (ss hyp_p) with ⟨s, hyp_s⟩,
@@ -362,141 +219,141 @@ begin
   { refine λ _ _ _, ⟨0, by simp⟩ }
 end
 
-@[simp] lemma dne (p) : T ⊢̇ ¬̇¬̇p →̇ p :=
+@[simp] lemma dne (p) : T ⊢ ¬̇¬̇p →̇ p :=
 begin
-  have lmm₁ : T+{¬̇¬̇p} ⊢̇ ¬̇¬̇p, simp,   
-  have lmm₂ : T+{¬̇¬̇p} ⊢̇ ¬̇¬̇p →̇ ¬̇¬̇¬̇¬̇p →̇ ¬̇¬̇p, simp,
-  have lmm₃ : T+{¬̇¬̇p} ⊢̇ ¬̇¬̇¬̇¬̇p →̇ ¬̇¬̇p, from lmm₂.MP lmm₁,
-  have lmm₄ : T+{¬̇¬̇p} ⊢̇ (¬̇¬̇¬̇¬̇p →̇ ¬̇¬̇p) →̇ ¬̇p →̇ ¬̇¬̇¬̇p, simp,
-  have lmm₅ : T+{¬̇¬̇p} ⊢̇ ¬̇p →̇ ¬̇¬̇¬̇p, from lmm₄.MP lmm₃,
-  have lmm₆ : T+{¬̇¬̇p} ⊢̇ (¬̇p →̇ ¬̇¬̇¬̇p) →̇ ¬̇¬̇p →̇ p, simp,
-  have lmm₇ : T+{¬̇¬̇p} ⊢̇ ¬̇¬̇p →̇ p, from lmm₆.MP lmm₅,
-  have lmm₈ : T+{¬̇¬̇p} ⊢̇ p, from lmm₇.MP lmm₁,
+  have lmm₁ : T+{¬̇¬̇p} ⊢ ¬̇¬̇p, simp,   
+  have lmm₂ : T+{¬̇¬̇p} ⊢ ¬̇¬̇p →̇ ¬̇¬̇¬̇¬̇p →̇ ¬̇¬̇p, simp,
+  have lmm₃ : T+{¬̇¬̇p} ⊢ ¬̇¬̇¬̇¬̇p →̇ ¬̇¬̇p, from lmm₂.MP lmm₁,
+  have lmm₄ : T+{¬̇¬̇p} ⊢ (¬̇¬̇¬̇¬̇p →̇ ¬̇¬̇p) →̇ ¬̇p →̇ ¬̇¬̇¬̇p, simp,
+  have lmm₅ : T+{¬̇¬̇p} ⊢ ¬̇p →̇ ¬̇¬̇¬̇p, from lmm₄.MP lmm₃,
+  have lmm₆ : T+{¬̇¬̇p} ⊢ (¬̇p →̇ ¬̇¬̇¬̇p) →̇ ¬̇¬̇p →̇ p, simp,
+  have lmm₇ : T+{¬̇¬̇p} ⊢ ¬̇¬̇p →̇ p, from lmm₆.MP lmm₅,
+  have lmm₈ : T+{¬̇¬̇p} ⊢ p, from lmm₇.MP lmm₁,
   exact deduction.mp lmm₈  
 end
 
-@[simp] lemma dni (p) : T ⊢̇ p →̇ ¬̇¬̇p :=
-by { have : T ⊢̇ (¬̇¬̇¬̇p →̇ ¬̇p) →̇ p →̇ ¬̇¬̇p, simp,
+@[simp] lemma dni (p) : T ⊢ p →̇ ¬̇¬̇p :=
+by { have : T ⊢ (¬̇¬̇¬̇p →̇ ¬̇p) →̇ p →̇ ¬̇¬̇p, simp,
      exact this.MP (by simp) }
 
-@[simp] lemma dn_iff {p} : T ⊢̇ ¬̇¬̇p ↔ T ⊢̇ p :=
-⟨λ h, (show T ⊢̇ ¬̇¬̇p →̇ p, by simp).MP h, λ h,(show T ⊢̇ p →̇ ¬̇¬̇p, by simp).MP h⟩
+@[simp] lemma dn_iff {p} : T ⊢ ¬̇¬̇p ↔ T ⊢ p :=
+⟨λ h, (show T ⊢ ¬̇¬̇p →̇ p, by simp).MP h, λ h,(show T ⊢ p →̇ ¬̇¬̇p, by simp).MP h⟩
 
-@[simp] lemma dn1_iff {p q} : (T ⊢̇ ¬̇¬̇p →̇ q) ↔ (T ⊢̇ p →̇ q) :=
+@[simp] lemma dn1_iff {p q} : (T ⊢ ¬̇¬̇p →̇ q) ↔ (T ⊢ p →̇ q) :=
 ⟨(dni _).imp_trans, (dne _).imp_trans⟩
 
-@[simp] lemma dn2_iff {p q} : (T ⊢̇ p →̇ ¬̇¬̇q) ↔ (T ⊢̇ p →̇ q) :=
+@[simp] lemma dn2_iff {p q} : (T ⊢ p →̇ ¬̇¬̇q) ↔ (T ⊢ p →̇ q) :=
 ⟨λ h, h.imp_trans (dne _), λ h, h.imp_trans (dni _)⟩
 
-lemma explosion {p} (h₁ : T ⊢̇ p) (h₂ : T ⊢̇ ¬̇p) {q} : T ⊢̇ q :=
+lemma explosion {p} (h₁ : T ⊢ p) (h₂ : T ⊢ ¬̇p) {q} : T ⊢ q :=
 begin
-  have : T ⊢̇ ¬̇p →̇ ¬̇q →̇ ¬̇p, simp,
-  have : T ⊢̇ ¬̇q →̇ ¬̇p, from this.MP h₂,
-  have : T ⊢̇ p →̇ q, from (show T ⊢̇ (¬̇q →̇ ¬̇p) →̇ p →̇ q, by simp).MP this,
+  have : T ⊢ ¬̇p →̇ ¬̇q →̇ ¬̇p, simp,
+  have : T ⊢ ¬̇q →̇ ¬̇p, from this.MP h₂,
+  have : T ⊢ p →̇ q, from (show T ⊢ (¬̇q →̇ ¬̇p) →̇ p →̇ q, by simp).MP this,
   exact this.MP h₁
 end
 
-lemma contrapose {p q} : (T ⊢̇ ¬̇p →̇ ¬̇q) ↔ (T ⊢̇ q →̇ p) :=
-⟨λ h, (show T ⊢̇ (¬̇p →̇ ¬̇q) →̇ q →̇ p, by simp).MP h, λ h,
-  by { refine (show T ⊢̇ (¬̇¬̇q →̇ ¬̇¬̇p) →̇ ¬̇p →̇ ¬̇q, by simp).MP _,
-       have : T ⊢̇ ¬̇¬̇q →̇ p, from (show T ⊢̇ ¬̇¬̇q →̇ q, by simp).imp_trans h,
-       exact this.imp_trans (show T ⊢̇ p →̇ ¬̇¬̇p, by simp) }⟩
+lemma contrapose {p q} : (T ⊢ ¬̇p →̇ ¬̇q) ↔ (T ⊢ q →̇ p) :=
+⟨λ h, (show T ⊢ (¬̇p →̇ ¬̇q) →̇ q →̇ p, by simp).MP h, λ h,
+  by { refine (show T ⊢ (¬̇¬̇q →̇ ¬̇¬̇p) →̇ ¬̇p →̇ ¬̇q, by simp).MP _,
+       have : T ⊢ ¬̇¬̇q →̇ p, from (show T ⊢ ¬̇¬̇q →̇ q, by simp).imp_trans h,
+       exact this.imp_trans (show T ⊢ p →̇ ¬̇¬̇p, by simp) }⟩
 
-lemma neg_hyp {p} (h : T ⊢̇ p →̇ ¬̇p) : T ⊢̇ ¬̇p :=
+lemma neg_hyp {p} (h : T ⊢ p →̇ ¬̇p) : T ⊢ ¬̇p :=
 begin
-  have : T+{p} ⊢̇ ¬̇(p →̇ ¬̇p),
-  { have lmm₁ : T+{p} ⊢̇ p, simp,
-    have lmm₂ : T+{p} ⊢̇ ¬̇p, from (weakening h _).MP lmm₁,
+  have : T+{p} ⊢ ¬̇(p →̇ ¬̇p),
+  { have lmm₁ : T+{p} ⊢ p, simp,
+    have lmm₂ : T+{p} ⊢ ¬̇p, from (weakening h _).MP lmm₁,
     exact explosion lmm₁ lmm₂ },
-  have : T ⊢̇ p →̇ ¬̇(p →̇ ¬̇p), from deduction.mp this,
-  have : T ⊢̇ (p →̇ ¬̇p) →̇ ¬̇p, from (dni _).imp_trans (contrapose.mpr this),
+  have : T ⊢ p →̇ ¬̇(p →̇ ¬̇p), from deduction.mp this,
+  have : T ⊢ (p →̇ ¬̇p) →̇ ¬̇p, from (dni _).imp_trans (contrapose.mpr this),
   exact this.MP h
 end
 
-lemma raa {p} (q) (h₁ : T+{p} ⊢̇ q) (h₂ : T+{p} ⊢̇ ¬̇q) : T ⊢̇ ¬̇p :=
+lemma raa {p} (q) (h₁ : T+{p} ⊢ q) (h₂ : T+{p} ⊢ ¬̇q) : T ⊢ ¬̇p :=
 neg_hyp (deduction.mp (explosion h₁ h₂))
 
-@[simp] lemma hyp_bot (p) : T ⊢̇ ⊥̇ →̇ p :=
-by { simp[formula.bot], apply deduction.mp, refine explosion (show T+{¬̇⊤̇} ⊢̇ ⊤̇, by simp) (add _ _) }
+@[simp] lemma hyp_bot (p) : T ⊢ ⊥̇ →̇ p :=
+by { simp[formula.bot], apply deduction.mp, refine explosion (show T+{¬̇⊤̇} ⊢ ⊤̇, by simp) (add _ _) }
 
-@[simp] lemma and {p q} : (T ⊢̇ p ⩑ q) ↔ (T ⊢̇ p ∧ T ⊢̇ q) :=
+@[simp] lemma and {p q} : (T ⊢ p ⩑ q) ↔ (T ⊢ p ∧ T ⊢ q) :=
 ⟨λ h, by { simp[formula.and] at h, split,
-   { have : T+{¬̇p}+{p} ⊢̇ ¬̇q, 
-     from explosion (show T+{¬̇p}+{p} ⊢̇ p, by simp) (show T+{¬̇p}+{p} ⊢̇ ¬̇p, by simp),
-     have : T ⊢̇ ¬̇p →̇ p →̇ ¬̇q, from (deduction.mp (deduction.mp this)),
-     have : T ⊢̇ ¬̇(p →̇ ¬̇q) →̇ p := (contrapose.mpr this).imp_trans (by simp),
+   { have : T+{¬̇p}+{p} ⊢ ¬̇q, 
+     from explosion (show T+{¬̇p}+{p} ⊢ p, by simp) (show T+{¬̇p}+{p} ⊢ ¬̇p, by simp),
+     have : T ⊢ ¬̇p →̇ p →̇ ¬̇q, from (deduction.mp (deduction.mp this)),
+     have : T ⊢ ¬̇(p →̇ ¬̇q) →̇ p := (contrapose.mpr this).imp_trans (by simp),
      exact this.MP h },
-   { have : T ⊢̇ ¬̇q →̇ p →̇ ¬̇q, simp,
-     have : T ⊢̇ ¬̇(p →̇ ¬̇q) →̇ q, from (contrapose.mpr this).imp_trans (by simp),
+   { have : T ⊢ ¬̇q →̇ p →̇ ¬̇q, simp,
+     have : T ⊢ ¬̇(p →̇ ¬̇q) →̇ q, from (contrapose.mpr this).imp_trans (by simp),
      exact this.MP h } },
  λ h, by {simp[formula.and], rcases h with ⟨h₁, h₂⟩,
-   show T ⊢̇ ¬̇(p →̇ ¬̇q),
-   have : T+{p →̇ ¬̇q} ⊢̇ ¬̇q, from (add _ _).MP (by simp[h₁]),
-   have : T ⊢̇ (p →̇ ¬̇q) →̇ ¬̇q, from deduction.mp this,
-   have : T ⊢̇ q →̇ ¬̇(p →̇ ¬̇q), from (dni _).imp_trans (contrapose.mpr this),
+   show T ⊢ ¬̇(p →̇ ¬̇q),
+   have : T+{p →̇ ¬̇q} ⊢ ¬̇q, from (add _ _).MP (by simp[h₁]),
+   have : T ⊢ (p →̇ ¬̇q) →̇ ¬̇q, from deduction.mp this,
+   have : T ⊢ q →̇ ¬̇(p →̇ ¬̇q), from (dni _).imp_trans (contrapose.mpr this),
    exact this.MP h₂ }⟩
 
-@[simp] lemma iff {p q} : (T ⊢̇ p ↔̇ q) ↔ (T ⊢̇ p →̇ q ∧ T ⊢̇ q →̇ p) :=
+@[simp] lemma iff {p q} : (T ⊢ p ↔̇ q) ↔ (T ⊢ p →̇ q ∧ T ⊢ q →̇ p) :=
 by simp[formula.iff]
 
-@[simp] lemma neg_imp {p q} : (T ⊢̇ ¬̇(p →̇ q)) ↔ (T ⊢̇ p ⩑ ¬̇q) :=
+@[simp] lemma neg_imp {p q} : (T ⊢ ¬̇(p →̇ q)) ↔ (T ⊢ p ⩑ ¬̇q) :=
 begin
   simp only [formula.and], split; intros h,
   { apply raa (p →̇ q),
-    { have : T+{p →̇ ¬̇¬̇q} ⊢̇ p →̇ ¬̇¬̇q, from add _ _, simp* at * },
+    { have : T+{p →̇ ¬̇¬̇q} ⊢ p →̇ ¬̇¬̇q, from add _ _, simp* at * },
     { simp[h] } },
   { apply raa (p →̇ ¬̇¬̇q); simp[h] }
 end
 
-lemma or_l (p q) : T ⊢̇ p →̇ p ⩒ q :=
-by simp[formula.or]; refine deduction.mp (deduction.mp (explosion (show T+{p}+{¬̇p} ⊢̇ p, by simp) (by simp)))
+lemma or_l (p q) : T ⊢ p →̇ p ⩒ q :=
+by simp[formula.or]; refine deduction.mp (deduction.mp (explosion (show T+{p}+{¬̇p} ⊢ p, by simp) (by simp)))
 
-lemma or_r (p q) : T ⊢̇ q →̇ p ⩒ q :=
+lemma or_r (p q) : T ⊢ q →̇ p ⩒ q :=
 by simp[formula.or]; refine deduction.mp (weakening h _)
 
-lemma hyp_or {p₁ p₂ q} : (T ⊢̇ p₁ →̇ q) → (T ⊢̇ p₂ →̇ q) → (T ⊢̇ p₁ ⩒ p₂ →̇ q) := λ h₁ h₂,
+lemma hyp_or {p₁ p₂ q} : (T ⊢ p₁ →̇ q) → (T ⊢ p₂ →̇ q) → (T ⊢ p₁ ⩒ p₂ →̇ q) := λ h₁ h₂,
 begin
   simp[formula.or], apply contrapose.mp, refine deduction.mp _, simp,
   refine ⟨deduction.mpr (contrapose.mpr h₁), deduction.mpr (contrapose.mpr h₂)⟩, 
 end
 
-lemma hyp_and_left {p₁ p₂ q} : (T ⊢̇ p₁ →̇ q) → (T ⊢̇ p₁ ⩑ p₂ →̇ q) := λ h,
+lemma hyp_and_left {p₁ p₂ q} : (T ⊢ p₁ →̇ q) → (T ⊢ p₁ ⩑ p₂ →̇ q) := λ h,
 begin
-  have : T+{p₁ ⩑ p₂} ⊢̇ p₁, { have : T+{p₁ ⩑ p₂} ⊢̇ p₁ ⩑ p₂, from add _ _, simp* at * },
-  refine deduction.mp ((show T+{p₁ ⩑ p₂} ⊢̇ p₁ →̇ q, by simp[h]).MP this)
+  have : T+{p₁ ⩑ p₂} ⊢ p₁, { have : T+{p₁ ⩑ p₂} ⊢ p₁ ⩑ p₂, from add _ _, simp* at * },
+  refine deduction.mp ((show T+{p₁ ⩑ p₂} ⊢ p₁ →̇ q, by simp[h]).MP this)
 end
 
-lemma hyp_and_right {p₁ p₂ q} : (T ⊢̇ p₂ →̇ q) → (T ⊢̇ p₁ ⩑ p₂ →̇ q) := λ h,
+lemma hyp_and_right {p₁ p₂ q} : (T ⊢ p₂ →̇ q) → (T ⊢ p₁ ⩑ p₂ →̇ q) := λ h,
 begin
-  have : T+{p₁ ⩑ p₂} ⊢̇ p₂, { have : T+{p₁ ⩑ p₂} ⊢̇ p₁ ⩑ p₂, from add _ _, simp* at * },
-  refine deduction.mp ((show T+{p₁ ⩑ p₂} ⊢̇ p₂ →̇ q, by simp[h]).MP this)
+  have : T+{p₁ ⩑ p₂} ⊢ p₂, { have : T+{p₁ ⩑ p₂} ⊢ p₁ ⩑ p₂, from add _ _, simp* at * },
+  refine deduction.mp ((show T+{p₁ ⩑ p₂} ⊢ p₂ →̇ q, by simp[h]).MP this)
 end
 
-lemma axiom_and {p₁ p₂ q} : T+{p₁ ⩑ p₂} ⊢̇ q ↔ T+{p₁}+{p₂} ⊢̇ q :=
+lemma axiom_and {p₁ p₂ q} : T+{p₁ ⩑ p₂} ⊢ q ↔ T+{p₁}+{p₂} ⊢ q :=
 ⟨λ h,
- by { have lmm₁ : T+{p₁}+{p₂} ⊢̇ p₁ ⩑ p₂, by simp,
-      have lmm₂ : T+{p₁}+{p₂} ⊢̇ p₁ ⩑ p₂ →̇ q, simp[deduction.mp h],
+ by { have lmm₁ : T+{p₁}+{p₂} ⊢ p₁ ⩑ p₂, by simp,
+      have lmm₂ : T+{p₁}+{p₂} ⊢ p₁ ⩑ p₂ →̇ q, simp[deduction.mp h],
       exact lmm₂.MP lmm₁ },
  λ h,
- by { have lmm₁ : T+{p₁ ⩑ p₂} ⊢̇ p₁ →̇ p₂ →̇ q, simp[deduction.mp (deduction.mp h)],
-      have lmm₂ : T+{p₁ ⩑ p₂} ⊢̇ p₁ ⩑ p₂, from add _ _, simp at lmm₂,
+ by { have lmm₁ : T+{p₁ ⩑ p₂} ⊢ p₁ →̇ p₂ →̇ q, simp[deduction.mp (deduction.mp h)],
+      have lmm₂ : T+{p₁ ⩑ p₂} ⊢ p₁ ⩑ p₂, from add _ _, simp at lmm₂,
       exact (lmm₁.MP lmm₂.1).MP lmm₂.2 }  ⟩
 
-lemma conjunction_mem {P : list (formula L)} : ∀ {p}, p ∈ P → ∅ ⊢̇ conjunction P →̇ p :=
+lemma conjunction_mem {P : list (formula L)} : ∀ {p}, p ∈ P → ∅ ⊢ conjunction P →̇ p :=
 begin
   induction P with p P IH; simp[conjunction],
-  have lmm₁ : ∅ ⊢̇ p ⩑ conjunction P →̇ p, from hyp_and_left (by simp),
-  have lmm₂ : ∀ q, q ∈ P → ∅ ⊢̇ p ⩑ conjunction P →̇ q, from λ q hq, hyp_and_right (IH hq),
+  have lmm₁ : ∅ ⊢ p ⩑ conjunction P →̇ p, from hyp_and_left (by simp),
+  have lmm₂ : ∀ q, q ∈ P → ∅ ⊢ p ⩑ conjunction P →̇ q, from λ q hq, hyp_and_right (IH hq),
   refine ⟨lmm₁, lmm₂⟩
 end
 
 lemma conjunction_inclusion {P Q : list (formula L)} : 
-  Q ⊆ P → ∅ ⊢̇ conjunction P →̇ conjunction Q :=
+  Q ⊆ P → ∅ ⊢ conjunction P →̇ conjunction Q :=
 begin
   induction Q with q Q IH; simp[conjunction],
   intros hyp_q hyp_Q,
-  have lmm₁ : ∅+{conjunction P} ⊢̇ q, from deduction.mpr (conjunction_mem hyp_q),  
-  have lmm₂ : ∅+{conjunction P} ⊢̇ conjunction Q, from deduction.mpr (IH hyp_Q),
+  have lmm₁ : ∅+{conjunction P} ⊢ q, from deduction.mpr (conjunction_mem hyp_q),  
+  have lmm₂ : ∅+{conjunction P} ⊢ conjunction Q, from deduction.mpr (IH hyp_Q),
   refine deduction.mp (and.mpr ⟨lmm₁, lmm₂⟩)
 end
 
@@ -509,7 +366,7 @@ begin
     { intros p hyp_p, refine hyp _ _, simp[hyp_p] },
     rcases IHl this with ⟨P, hyp_P⟩,
     have := hyp p₀ (by simp),
-    cases this with p hyp_p,
+    rcases this with ⟨p, hyp_p, rfl⟩,
     have lmm₁ : (conjunction (p :: P)).sf = conjunction (p.sf :: P₀),
     { simp[conjunction, hyp_P] },
     have lmm₂ : ∀ (q : formula L), q ∈ (p :: P) → T q,
@@ -518,14 +375,14 @@ begin
 end
 
 theorem proof_conjunction {T : theory L} {p} :
-  T ⊢̇ p → ∃ P : list (formula L), (∀ p, p ∈ P → T p) ∧ ∅ ⊢̇ conjunction P →̇ p := λ h,
+  T ⊢ p → ∃ P : list (formula L), (∀ p, p ∈ P → T p) ∧ ∅ ⊢ conjunction P →̇ p := λ h,
 begin
   induction h,
   case fopl.provable.GE : T p hyp IH
   { rcases IH with ⟨P₀, hyp_P₀, prov⟩,
     have : ∃ P, (conjunction P).sf = conjunction P₀ ∧ ∀ p, p ∈ P → T p, from conjunction_sf _ hyp_P₀,
     rcases this with ⟨P, eqn, hyp_P⟩,
-    have : ∅ ⊢̇ conjunction P →̇ ∀̇p,
+    have : ∅ ⊢ conjunction P →̇ ∀̇p,
     { refine deduction.mp (GE _),
       rw [←sf_dsb, eqn], refine deduction.mpr (inclusion prov (λ x hx, _)), cases hx },
     refine ⟨P, hyp_P, this⟩ },
@@ -533,16 +390,16 @@ begin
   { rcases IH₁ with ⟨P₁, IH₁, prov₁⟩, rcases IH₂ with ⟨P₂, IH₂, prov₂⟩,
     refine ⟨P₁ ++ P₂, _, _⟩,
     { simp, intros p h, cases h, refine IH₁ _ h, refine IH₂ _ h },
-    { have : ∅+{conjunction (P₁ ++ P₂)} ⊢̇ conjunction P₂, from deduction.mpr (conjunction_inclusion (by simp)),
-      have lmm₁ : ∅+{conjunction (P₁ ++ P₂)} ⊢̇ p, from (show _ ⊢̇ conjunction P₂ →̇ p, by simp[prov₂]).MP this,
-      have : ∅+{conjunction (P₁ ++ P₂)} ⊢̇ conjunction P₁, from deduction.mpr (conjunction_inclusion (by simp)),
-      have lmm₂ : ∅+{conjunction (P₁ ++ P₂)} ⊢̇ p →̇ q,
-      from (show _ ⊢̇ conjunction P₁ →̇ p →̇ q, by simp[prov₁]).MP this,
+    { have : ∅+{conjunction (P₁ ++ P₂)} ⊢ conjunction P₂, from deduction.mpr (conjunction_inclusion (by simp)),
+      have lmm₁ : ∅+{conjunction (P₁ ++ P₂)} ⊢ p, from (show _ ⊢ conjunction P₂ →̇ p, by simp[prov₂]).MP this,
+      have : ∅+{conjunction (P₁ ++ P₂)} ⊢ conjunction P₁, from deduction.mpr (conjunction_inclusion (by simp)),
+      have lmm₂ : ∅+{conjunction (P₁ ++ P₂)} ⊢ p →̇ q,
+      from (show _ ⊢ conjunction P₁ →̇ p →̇ q, by simp[prov₁]).MP this,
       refine deduction.mp (lmm₂.MP lmm₁) } },
   case fopl.provable.AX : T p hyp_p
   { refine ⟨[p], _⟩, simp[conjunction],
-    have : ∅ ⊢̇ p ⩑ ⊤̇ →̇ p,
-    { apply deduction.mp, have : ∅+{p ⩑ ⊤̇} ⊢̇ p ⩑ ⊤̇, from add _ _ , simp* at* },
+    have : ∅ ⊢ p ⩑ ⊤̇ →̇ p,
+    { apply deduction.mp, have : ∅+{p ⩑ ⊤̇} ⊢ p ⩑ ⊤̇, from add _ _ , simp* at* },
     refine ⟨hyp_p, this⟩ },
   { refine ⟨[], _⟩, simp },
   { refine ⟨[], _⟩, simp },
@@ -557,24 +414,24 @@ begin
   { refine ⟨[], _⟩, simp }
 end
 
-lemma fal_subst {p} (h : T ⊢̇ ∀̇p) (t) : T ⊢̇ p.rew ₛ[t] :=
-(show T ⊢̇ ∀̇p →̇ p.rew ₛ[t], by simp).MP h
+lemma fal_subst {p} (h : T ⊢ ∀̇p) (t) : T ⊢ p.rew ₛ[t] :=
+(show T ⊢ ∀̇p →̇ p.rew ₛ[t], by simp).MP h
 
-lemma add_sf (p) : ⇑(T +{∀̇p}) ⊢̇ p :=
-by { have : ⇑(T +{∀̇p}) ⊢̇ (∀̇p).sf, rw ← sf_dsb, simp,simp[formula.sf] at this,
+lemma add_sf (p) : ⇑(T +{∀̇p}) ⊢ p :=
+by { have : ⇑(T +{∀̇p}) ⊢ (∀̇p).sf, rw ← sf_dsb, simp,simp[formula.sf] at this,
      have := fal_subst this #0, simp[formula.nested_rew] at this,
      have eqn : (λ x, vecterm.rew ₛ[#0] (((λ x, #(x + 1) : ℕ → term _)^1) x)) = (idvar : ℕ → vecterm L 0),
       { funext n, cases n; refl }, simp [eqn] at this, exact this }
 
-private lemma rgerg {P : list (formula L)} : (∀ p, p ∈ P → T p) → T ⊢̇ conjunction P :=
+private lemma rgerg {P : list (formula L)} : (∀ p, p ∈ P → T p) → T ⊢ conjunction P :=
 begin
   induction P with p P IH; simp[conjunction],
   refine λ hyp_p hyp, ⟨AX hyp_p, IH hyp⟩,
 end
 
-lemma cl_prove_rew [cl : closed_theory T] : ∀ {p : formula L}, T ⊢̇ p → ∀ s, T ⊢̇ p.rew s :=
+lemma cl_prove_rew [cl : closed_theory T] : ∀ {p : formula L}, T ⊢ p → ∀ s, T ⊢ p.rew s :=
 begin
-  suffices : ∀ {p : formula L} {T}, T ⊢̇ p → closed_theory T → ∀ s, T ⊢̇ p.rew s,
+  suffices : ∀ {p : formula L} {T}, T ⊢ p → closed_theory T → ∀ s, T ⊢ p.rew s,
   { refine λ p h s, this h cl _ },
   intros p T h,
   induction h,
@@ -603,16 +460,16 @@ begin
 end
 
 lemma pp_prove_rew {n} (pp : proper_at n T) :
-  ∀ {p : formula L}, T ⊢̇ p → ∀ s, T ⊢̇ p.rew (rewriting_sf_itr s n) :=
+  ∀ {p : formula L}, T ⊢ p → ∀ s, T ⊢ p.rew (s^n) :=
 begin
   suffices : ∀ {p : formula L} {T},
-    T ⊢̇ p → ∀ {n}, proper_at n T → ∀ s, T ⊢̇ p.rew (rewriting_sf_itr s n),
+    T ⊢ p → ∀ {n}, proper_at n T → ∀ s, T ⊢ p.rew (rewriting_sf_itr s n),
   { refine λ p h s, this h @pp _ },
   intros p T h,
   induction h,
   case GE : T p hyp IH
   { intros n pp s,
-    refine GE _, refine @IH (n+1) (@proper_theory_sf _ _ _ @pp) s },
+    refine GE _, refine @IH (n+1) (@proper_theory_sf_itr _ _ _ @pp 1) s },
   case MP : T p q hyp_pq hyp_p IH₁ IH₂
   { intros n pp s, refine (IH₁ @pp _).MP (IH₂ @pp _) },
   case AX : T p hyp
@@ -633,14 +490,14 @@ begin
 end
 
 lemma ppc_prove_rew (n) [pp : proper n T] :
-  ∀ {p : formula L}, T ⊢̇ p → ∀ s, T ⊢̇ p.rew (rewriting_sf_itr s n) := @pp_prove_rew _ _ n pp.proper
+  ∀ {p : formula L}, T ⊢ p → ∀ s, T ⊢ p.rew (s^n) := @pp_prove_rew _ _ n pp.proper
 
 lemma ppc0_prove_rew [pp : proper 0 T] :
-  ∀ {p : formula L}, T ⊢̇ p → ∀ s, T ⊢̇ p.rew s := @pp_prove_rew _ _ 0 pp.proper
+  ∀ {p : formula L}, T ⊢ p → ∀ s, T ⊢ p.rew s := @pp_prove_rew _ _ 0 pp.proper
 
-lemma cl_fal_elim [closed_theory T] {p} : T ⊢̇ ∀̇p ↔ T ⊢̇ p :=
-⟨λ h, by { have : T ⊢̇ (∀̇p).rew (λ n, #(n+1)),  from cl_prove_rew h _,
-           have lmm : T ⊢̇ (p.rew (#0 ^ˢ λ n, #(n+2))).rew ₛ[#0], from this.fal_subst #0,
+lemma cl_fal_elim [closed_theory T] {p} : T ⊢ ∀̇p ↔ T ⊢ p :=
+⟨λ h, by { have : T ⊢ (∀̇p).rew (λ n, #(n+1)),  from cl_prove_rew h _,
+           have lmm : T ⊢ (p.rew (#0 ^ˢ λ n, #(n+2))).rew ₛ[#0], from this.fal_subst #0,
            have : (p.rew (#0 ^ˢ λ n, #(n+2))).rew ₛ[#0] = p,
            { suffices : (p.rew (#0 ^ˢ λ n, #(n+2))).rew ₛ[#0] = p.rew idvar, simp* at*,
              simp[formula.nested_rew, -formula.rew_idvar], congr,
@@ -653,35 +510,35 @@ private lemma conjunction_rew_eq : ∀ (P : list (formula L)) (s),
 | []       _ := by simp[conjunction, formula.rew]
 | (p :: P) s := by simp[conjunction, formula.rew, conjunction_rew_eq P]
 
-lemma conjunction_provable : ∀ {P : list (formula L)} (h : ∀ p, p ∈ P → T ⊢̇ p), T ⊢̇ conjunction P
+lemma conjunction_provable : ∀ {P : list (formula L)} (h : ∀ p, p ∈ P → T ⊢ p), T ⊢ conjunction P
 | []       h := by simp[conjunction]
 | (p :: P) h := by { simp[conjunction],
-    have lmm₁ : T ⊢̇ p, { refine h _ _, simp },
-    have lmm₂ : T ⊢̇ conjunction P, { refine conjunction_provable (λ p hyp, h _ _), simp, right, exact hyp },
+    have lmm₁ : T ⊢ p, { refine h _ _, simp },
+    have lmm₂ : T ⊢ conjunction P, { refine conjunction_provable (λ p hyp, h _ _), simp, right, exact hyp },
     refine ⟨lmm₁, lmm₂⟩ }
 
-lemma sf_sf {p : formula L} : ⇑T ⊢̇ p.sf ↔ T ⊢̇ p :=
+lemma sf_sf {p : formula L} : ⇑T ⊢ p.sf ↔ T ⊢ p :=
 ⟨λ h, by { have := (GE h).fal_subst #0, simp* at* },
- λ h, by { have : ∃ P, (∀ p, p ∈ P → p ∈ T) ∧ ∅ ⊢̇ conjunction P →̇ p,
+ λ h, by { have : ∃ P, (∀ p, p ∈ P → p ∈ T) ∧ ∅ ⊢ conjunction P →̇ p,
   from proof_conjunction h, rcases this with ⟨P, hyp_P, prov⟩,
-  have lmm₁ : ⇑T ⊢̇ conjunction (P.map formula.sf),
+  have lmm₁ : ⇑T ⊢ conjunction (P.map formula.sf),
   { refine conjunction_provable (λ p hyp, AX _), simp at hyp, rcases hyp with ⟨p', p'_mem, rfl⟩,
-    refine theory.sf.intro (hyp_P p' p'_mem) },
-  have lmm₂ : ⇑T ⊢̇ conjunction (P.map formula.sf) →̇ p.sf,
-  { have : ∅ ⊢̇ (conjunction P).sf →̇ p.sf, from cl_prove_rew prov _,
+    refine ⟨p', hyp_P p' p'_mem, rfl⟩ },
+  have lmm₂ : ⇑T ⊢ conjunction (P.map formula.sf) →̇ p.sf,
+  { have : ∅ ⊢ (conjunction P).sf →̇ p.sf, from cl_prove_rew prov _,
     simp[conjunction_rew_eq, formula.sf] at this,
     refine inclusion this (λ p h, _), exfalso, exact h },
   refine lmm₂.MP lmm₁ }⟩
 
 lemma sf_itr_sf_itr : ∀ {n} {p : formula L},
-  T^n ⊢̇ p.rew (λ x, #(x+n)) ↔ T ⊢̇ p
+  T^n ⊢ p.rew (λ x, #(x+n)) ↔ T ⊢ p
 | 0     p := by simp
 | (n+1) p := by { simp[←add_assoc],
     have : p.rew (λ x, #(x + n + 1)) = (p.rew (λ x, #(x+n))).sf,
     { simp[formula.sf, formula.nested_rew] }, simp[this, sf_sf],
     exact sf_itr_sf_itr }
 
-lemma use {p : formula L} (t) (h : T ⊢̇ p.rew ₛ[t]) : T ⊢̇ ∃̇p :=
+lemma use {p : formula L} (t) (h : T ⊢ p.rew ₛ[t]) : T ⊢ ∃̇p :=
 begin
   simp[formula.ex],
   refine raa (p.rew ₛ[t]) (by simp[h]) (deduction.mpr _),
@@ -689,20 +546,20 @@ begin
   rw[this], refine provable.q1
 end
 
-lemma eq_symm : ∀ {t u}, (T ⊢̇ t =̇ u) ↔ (T ⊢̇ u =̇ t) :=
+lemma eq_symm : ∀ {t u}, (T ⊢ t =̇ u) ↔ (T ⊢ u =̇ t) :=
 begin
-  suffices : ∀ t u, (T ⊢̇ t =̇ u) → (T ⊢̇ u =̇ t),
+  suffices : ∀ t u, (T ⊢ t =̇ u) → (T ⊢ u =̇ t),
   { intros t u, refine ⟨this _ _, this _ _⟩ },
   intros t u h,
-  have : T ⊢̇ t =̇ u →̇ u =̇ t, simp,
+  have : T ⊢ t =̇ u →̇ u =̇ t, simp,
   refine this.MP h
 end
 
-lemma eq_trans {t₁ t₂ t₃} : (T ⊢̇ t₁ =̇ t₂) → (T ⊢̇ t₂ =̇ t₃) → (T ⊢̇ t₁ =̇ t₃) := λ h₁ h₂,
-by { have : T ⊢̇ t₁ =̇ t₂ →̇ t₂ =̇ t₃ →̇ t₁ =̇ t₃, simp, exact (this.MP h₁).MP h₂ }
+lemma eq_trans {t₁ t₂ t₃} : (T ⊢ t₁ =̇ t₂) → (T ⊢ t₂ =̇ t₃) → (T ⊢ t₁ =̇ t₃) := λ h₁ h₂,
+by { have : T ⊢ t₁ =̇ t₂ →̇ t₂ =̇ t₃ →̇ t₁ =̇ t₃, simp, exact (this.MP h₁).MP h₂ }
 
-lemma equal_rew_equals : ∀ {n} (v : vecterm L n) (s₁ s₂ : ℕ → term L) (e : ∀ n, T ⊢̇ s₁ n =̇ s₂ n),
-  T ⊢̇ v.rew s₁ ≡̇ v.rew s₂
+lemma equal_rew_equals : ∀ {n} (v : vecterm L n) (s₁ s₂ : ℕ → term L) (e : ∀ n, T ⊢ s₁ n =̇ s₂ n),
+  T ⊢ v.rew s₁ ≡̇ v.rew s₂
 | _ (vecterm.cons t v) _ _ eqn := by simp[vecterm.rew];
     exact ⟨equal_rew_equals t _ _ eqn, equal_rew_equals v _ _ eqn⟩
 | _ (#n)               _ _ eqn := by simp[vecterm.rew]; exact eqn _
@@ -710,15 +567,15 @@ lemma equal_rew_equals : ∀ {n} (v : vecterm L n) (s₁ s₂ : ℕ → term L) 
 | _ (vecterm.app f v)  _ _ eqn := by simp[vecterm.rew];
     exact provable.e4.MP (equal_rew_equals v _ _ eqn)
 
-lemma equal_rew_equals_term : ∀ (t : term L) (s₁ s₂ : ℕ → term L) (e : ∀ n, T ⊢̇ s₁ n =̇ s₂ n),
-  T ⊢̇ t.rew s₁ =̇ t.rew s₂ := equal_rew_equals
+lemma equal_rew_equals_term : ∀ (t : term L) (s₁ s₂ : ℕ → term L) (e : ∀ n, T ⊢ s₁ n =̇ s₂ n),
+  T ⊢ t.rew s₁ =̇ t.rew s₂ := equal_rew_equals
 
-lemma equal_fal_subst_equals {n} (v : vecterm L n) {t₁ t₂} (h : T ⊢̇ t₁ =̇ t₂) :
-  T ⊢̇ v.rew (t₁ ^ˢ idvar) ≡̇ v.rew (t₂ ^ˢ idvar) :=
+lemma equal_fal_subst_equals {n} (v : vecterm L n) {t₁ t₂} (h : T ⊢ t₁ =̇ t₂) :
+  T ⊢ v.rew (t₁ ^ˢ idvar) ≡̇ v.rew (t₂ ^ˢ idvar) :=
 by { refine equal_rew_equals v _ _ (λ n, _), { cases n; simp[h] } }
 
-lemma equal_rew_iff (p : formula L) : ∀ {s₁ s₂ : ℕ → term L} {T : theory L} (eqn : ∀ n, T ⊢̇ s₁ n =̇ s₂ n),
-  T ⊢̇ p.rew s₁ ↔̇ p.rew s₂ :=
+lemma equal_rew_iff (p : formula L) : ∀ {s₁ s₂ : ℕ → term L} {T : theory L} (eqn : ∀ n, T ⊢ s₁ n =̇ s₂ n),
+  T ⊢ p.rew s₁ ↔̇ p.rew s₂ :=
 begin
   induction p,
   case const { by simp[formula.rew] },
@@ -727,32 +584,32 @@ begin
       (provable.e5.MP (equal_rew_equals v _ _ (λ n, eq_symm.mp $ eqn n)))⟩ },
   case equal : t₁ t₂ { intros, simp[formula.rew],
     refine ⟨deduction.mp _, deduction.mp _⟩,
-    { have lmm₁ : T+{t₁.rew s₁ =̇ t₂.rew s₁} ⊢̇ t₁.rew s₂ =̇ t₁.rew s₁,
+    { have lmm₁ : T+{t₁.rew s₁ =̇ t₂.rew s₁} ⊢ t₁.rew s₂ =̇ t₁.rew s₁,
       { refine equal_rew_equals t₁ s₂ s₁ (λ n, eq_symm.mp _), simp[eqn n] },
-      have lmm₂ : T+{t₁.rew s₁ =̇ t₂.rew s₁} ⊢̇ t₁.rew s₁ =̇ t₂.rew s₁, { simp },
-      have lmm₃ : T+{t₁.rew s₁ =̇ t₂.rew s₁} ⊢̇ t₂.rew s₁ =̇ t₂.rew s₂,
+      have lmm₂ : T+{t₁.rew s₁ =̇ t₂.rew s₁} ⊢ t₁.rew s₁ =̇ t₂.rew s₁, { simp },
+      have lmm₃ : T+{t₁.rew s₁ =̇ t₂.rew s₁} ⊢ t₂.rew s₁ =̇ t₂.rew s₂,
       { refine equal_rew_equals t₂ s₁ s₂ (λ n, _), simp[eqn n]  },
       refine lmm₁.eq_trans (lmm₂.eq_trans lmm₃) },
-    { have lmm₁ : T+{t₁.rew s₂ =̇ t₂.rew s₂} ⊢̇ t₁.rew s₁ =̇ t₁.rew s₂,
+    { have lmm₁ : T+{t₁.rew s₂ =̇ t₂.rew s₂} ⊢ t₁.rew s₁ =̇ t₁.rew s₂,
       { refine equal_rew_equals t₁ s₁ s₂ (λ n, _), simp[eqn n] },
-      have lmm₂ : T+{t₁.rew s₂ =̇ t₂.rew s₂} ⊢̇ t₁.rew s₂ =̇ t₂.rew s₂, { simp },
-      have lmm₃ : T+{t₁.rew s₂ =̇ t₂.rew s₂} ⊢̇ t₂.rew s₂ =̇ t₂.rew s₁,
+      have lmm₂ : T+{t₁.rew s₂ =̇ t₂.rew s₂} ⊢ t₁.rew s₂ =̇ t₂.rew s₂, { simp },
+      have lmm₃ : T+{t₁.rew s₂ =̇ t₂.rew s₂} ⊢ t₂.rew s₂ =̇ t₂.rew s₁,
       { refine equal_rew_equals t₂ s₂ s₁ (λ n, eq_symm.mp _), simp[eqn n]  },
       refine lmm₁.eq_trans (lmm₂.eq_trans lmm₃) } },
   case imply : p q IH₁ IH₂
   { intros, have IH₁ := IH₁ eqn, have IH₂ := IH₂ eqn,
     simp[formula.rew] at*, split,
     { refine deduction.mp (deduction.mp _), 
-      have : T+{p.rew s₁ →̇ q.rew s₁}+{p.rew s₂} ⊢̇ p.rew s₂, simp,
-      have : T+{p.rew s₁ →̇ q.rew s₁}+{p.rew s₂} ⊢̇ p.rew s₁, from MP (by simp[IH₁]) this,
-      have : T+{p.rew s₁ →̇ q.rew s₁}+{p.rew s₂} ⊢̇ q.rew s₁,
-        from MP (show _ ⊢̇ p.rew s₁ →̇ q.rew s₁, by simp) this,
+      have : T+{p.rew s₁ →̇ q.rew s₁}+{p.rew s₂} ⊢ p.rew s₂, simp,
+      have : T+{p.rew s₁ →̇ q.rew s₁}+{p.rew s₂} ⊢ p.rew s₁, from MP (by simp[IH₁]) this,
+      have : T+{p.rew s₁ →̇ q.rew s₁}+{p.rew s₂} ⊢ q.rew s₁,
+        from MP (show _ ⊢ p.rew s₁ →̇ q.rew s₁, by simp) this,
       from MP (by simp[IH₂]) this },
     { refine deduction.mp (deduction.mp _),
-      have : T+{p.rew s₂ →̇ q.rew s₂}+{p.rew s₁} ⊢̇ p.rew s₁, simp,
-      have : T+{p.rew s₂ →̇ q.rew s₂}+{p.rew s₁} ⊢̇ p.rew s₂, from MP (by simp[IH₁]) this,
-      have : T+{p.rew s₂ →̇ q.rew s₂}+{p.rew s₁} ⊢̇ q.rew s₂,
-        from MP (show _ ⊢̇ p.rew s₂ →̇ q.rew s₂, by simp) this,
+      have : T+{p.rew s₂ →̇ q.rew s₂}+{p.rew s₁} ⊢ p.rew s₁, simp,
+      have : T+{p.rew s₂ →̇ q.rew s₂}+{p.rew s₁} ⊢ p.rew s₂, from MP (by simp[IH₁]) this,
+      have : T+{p.rew s₂ →̇ q.rew s₂}+{p.rew s₁} ⊢ q.rew s₂,
+        from MP (show _ ⊢ p.rew s₂ →̇ q.rew s₂, by simp) this,
       from MP (by simp[IH₂]) this } },
   case neg : p IH
   { intros, simp[formula.rew] at*,
@@ -765,21 +622,21 @@ begin
     refine ⟨provable.q2.MP (GE this.1), provable.q2.MP (GE this.2)⟩ }
 end
 
-lemma dummy_fal_quantifir (p) : T ⊢̇ p ↔̇ ∀̇(p.sf) :=
-by { have : T ⊢̇ ∀̇p.sf →̇ p.sf.rew ₛ[#0], from provable.q1, simp* at * }
+lemma dummy_fal_quantifir (p) : T ⊢ p ↔̇ ∀̇(p.sf) :=
+by { have : T ⊢ ∀̇p.sf →̇ p.sf.rew ₛ[#0], from provable.q1, simp* at * }
 
-lemma dummy_fal_quantifir_iff {p : formula L} : T ⊢̇ ∀̇(p.sf) ↔ T ⊢̇ p :=
+lemma dummy_fal_quantifir_iff {p : formula L} : T ⊢ ∀̇(p.sf) ↔ T ⊢ p :=
 by { have := provable.iff.mp (@dummy_fal_quantifir _ T p), split,
      { refine λ h, (this.2.MP h) },
      { refine λ h, (this.1.MP h) } }
 
-lemma dummy_ex_quantifir (p) : T ⊢̇ p ↔̇ ∃̇(p.sf) :=
+lemma dummy_ex_quantifir (p) : T ⊢ p ↔̇ ∃̇ (p.sf) :=
 by { simp[formula.ex], split,
      { refine contrapose.mp _, simp, exact (provable.iff.mp (dummy_fal_quantifir ¬̇p)).2 },
      { refine contrapose.mp _, simp, exact (provable.iff.mp (dummy_fal_quantifir ¬̇p)).1 } }
 
-@[simp] lemma T_hyp_eliminate {p} : T ⊢̇ ⊤̇ →̇ p ↔ T ⊢̇ p :=
-⟨λ h, by { have : T ⊢̇ ⊤̇, simp, exact h.MP this }, λ h, by simp[h]⟩
+@[simp] lemma T_hyp_eliminate {p} : T ⊢ ⊤̇ →̇ p ↔ T ⊢ p :=
+⟨λ h, by { have : T ⊢ ⊤̇, simp, exact h.MP this }, λ h, by simp[h]⟩
 
 end provable
 
